Start the Indexed Coinduction.

theories/Eq/Eq.v
@@ -19,11 +19,14 @@ From Coq Require Import
      Program
      Setoid
      Morphisms
-     RelationClasses.
+     Relations
+     RelationClasses
+     Lia.
 
 From Paco Require Import paco.
 
 From ITree Require Import
+     Basics.GeneralWFO
      Basics.Basics
      Basics.HeterogeneousRelations
      Core.ITreeDefinition.
@@ -40,7 +43,32 @@ Proof. auto. Qed.
 
 Global Instance Transitive_bot2 (A : Type) : @Transitive A bot2.
 Proof. auto. Qed.
+
 (* end hide *)
+
+Hint Resolve wfo_lt_le_lt wfo_le_lt_lt wfo_le_le_le wfo_add_lt_left wfo_add_lt_right wfo_add_le_left wfo_add_le_right wfo_add_monotone wfo_lt_le : wfo.
+Hint Resolve wfo_add_proj_left wfo_add_proj_right : wfo_proj.
+Hint Resolve wfo_le_refl : wfo_refl.
+
+Definition _tmp_id_ T (e: T) := e.
+
+Ltac unfold_eta :=
+  repeat
+  match goal with
+  | |- context[@RetF ?a ?b ?c ?d] =>
+    change (@RetF a b c d) with (observe (go ((@_tmp_id_ _ (@RetF)) a b c d)))
+  | H: context[@RetF ?a ?b ?c ?d] |- _ =>
+    change (@RetF a b c d) with (observe (go ((@_tmp_id_ _ (@RetF)) a b c d))) in H
+  | |- context[@TauF ?a ?b ?c ?d] =>
+    change (@TauF a b c d) with (observe (go ((@_tmp_id_ _ (@TauF)) a b c d)))
+  | H: context[@TauF ?a ?b ?c ?d] |- _ =>
+    change (@TauF a b c d) with (observe (go ((@_tmp_id_ _ (@TauF)) a b c d))) in H
+  | |- context[@VisF ?a ?b ?c ?d ?e ?f] =>
+    change (@VisF a b c d e f) with (observe (go ((@_tmp_id_ _ (@VisF)) a b c d e f)))
+  | H: context[@VisF ?a ?b ?c ?d ?e ?f] |- _ =>
+    change (@VisF a b c d e f) with (observe (go ((@_tmp_id_ _ (@VisF)) a b c d e f))) in H
+  end;
+  unfold _tmp_id_ in *.
 
 (** ** Coinductive reasoning with Paco *)
 
@@ -64,7 +92,7 @@ Proof. auto. Qed.
 
 Coercion is_true : bool >-> Sortclass.
 
-Section eqit.
+Section eqit_Definition.
 
   (** Although the original motivation is to define an equivalence
       relation on [itree E R], we will generalize it into a
@@ -75,8 +103,8 @@ Section eqit.
       Then the desired equivalence relation is obtained by setting
       [RR := eq] (with [R1 = R2]).
    *)
-  Context {E : Type -> Type} {R1 R2 : Type} (RR : R1 -> R2 -> Prop).
-
+  Context {E : Type -> Type}.
+ 
   (** We also need to do some gymnastics to work around the
       two-layered definition of [itree]. We first define a
       relation transformer [eqitF] as an indexed inductive type
@@ -87,185 +115,218 @@ Section eqit.
       pattern-matching is not allowed on [itree].
    *)
 
-  Inductive eqitF (b1 b2: bool) vclo (sim : itree E R1 -> itree E R2 -> Prop) :
+  Variant eqitF (b1 b2: bool) {R1 R2} (RR: R1->R2->Prop) (sim : gwfo -> itree E R1 -> itree E R2 -> Prop) (o: gwfo) :
     itree' E R1 -> itree' E R2 -> Prop :=
   | EqRet r1 r2
-       (REL: RR r1 r2):
-     eqitF b1 b2 vclo sim (RetF r1) (RetF r2)
-  | EqTau m1 m2
-        (REL: sim m1 m2):
-      eqitF b1 b2 vclo sim (TauF m1) (TauF m2)
+        (REL: RR r1 r2)
+    : eqitF b1 b2 RR sim o (RetF r1) (RetF r2)
   | EqVis {u} (e : E u) k1 k2
-        (REL: forall v, vclo sim (k1 v) (k2 v) : Prop):
-      eqitF b1 b2 vclo sim (VisF e k1) (VisF e k2)
-  | EqTauL t1 ot2
-        (CHECK: b1)
-        (REL: eqitF b1 b2 vclo sim (observe t1) ot2):
-      eqitF b1 b2 vclo sim (TauF t1) ot2
-  | EqTauR ot1 t2
+        (REL: forall v, exists o', sim o' (k1 v) (k2 v))
+    : eqitF b1 b2 RR sim o (VisF e k1) (VisF e k2)
+  | EqTau m1 m2 o'
+        (REL: sim o' m1 m2)
+        (LEo: wfo_le o' o)
+    : eqitF b1 b2 RR sim o (TauF m1) (TauF m2)
+  | EqTauL t1 t2 o'
+        (CHECK: b1)           
+        (REL: sim o' t1 t2)          
+        (LTo: wfo_lt o' o)
+    : eqitF b1 b2 RR sim o (TauF t1) (observe t2)
+  | EqTauR t1 t2 o'
         (CHECK: b2)
-        (REL: eqitF b1 b2 vclo sim ot1 (observe t2)):
-      eqitF b1 b2 vclo sim ot1 (TauF t2)
+        (REL: sim o' t1 t2)           
+        (LTo: wfo_lt o' o)
+    : eqitF b1 b2 RR sim o (observe t1) (TauF t2)
+  | EqStutter t1 t2 o'
+        (CHECK1: b1)
+        (CHECK2: b2)
+        (REL: sim o' t1 t2)           
+        (LTo: wfo_lt o' o)
+    : eqitF b1 b2 RR sim o (observe t1) (observe t2)
   .
-  Hint Constructors eqitF: core.
+  
+  Definition eqit_ b1 b2
+             (sim: forall {R1 R2},(R1->R2->Prop)-> gwfo -> itree E R1 -> itree E R2 -> Prop)
+             R1 R2 (RR: R1->R2->Prop) o t1 t2 :=
+    eqitF b1 b2 RR (sim RR) o (observe t1) (observe t2).
 
-  Definition eqit_ b1 b2 vclo sim :
-    itree E R1 -> itree E R2 -> Prop :=
-    fun t1 t2 => eqitF b1 b2 vclo sim (observe t1) (observe t2).
-  Hint Unfold eqit_: core.
+  Definition eqiti b1 b2 {R1 R2} RR o t1 t2 :=
+    paco6 (eqit_ b1 b2) bot6 R1 R2 RR o t1 t2.
 
-  (** [eqitF] and [eqit_] are both monotone. *)
+  Definition eqitz b1 b2 {R1 R2} RR t1 t2 := @eqiti b1 b2 R1 R2 RR wfo_zero t1 t2.
 
-  Lemma eqitF_mono b1 b2 x0 x1 vclo vclo' sim sim'
-        (IN: eqitF b1 b2 vclo sim x0 x1)
-        (MON: monotone2 vclo)
-        (LEc: vclo <3= vclo')
-        (LE: sim <2= sim'):
-    eqitF b1 b2 vclo' sim' x0 x1.
-  Proof.
-    intros. induction IN; eauto.
-  Qed.
+  Variant eqit b1 b2 {R1 R2} RR t1 t2 : Prop :=
+  | eqit_exists o (REL: @eqiti b1 b2 R1 R2 RR o t1 t2)
+  .
 
-  Lemma eqit__mono b1 b2 vclo (MON: monotone2 vclo) : monotone2 (eqit_ b1 b2 vclo).
-  Proof. do 2 red. intros. eapply eqitF_mono; eauto. Qed.
-
-  Hint Resolve eqit__mono : paco.
-
-  Lemma eqit_idclo_mono: monotone2 (@id (itree E R1 -> itree E R2 -> Prop)).
-  Proof. unfold id. eauto. Qed.
-
-  Hint Resolve eqit_idclo_mono : paco.
-
-  Definition eqit b1 b2 : itree E R1 -> itree E R2 -> Prop :=
-    paco2 (eqit_ b1 b2 id) bot2.
-
-  (** Strong bisimulation on itrees. If [eqit RR t1 t2],
+  (** Strong bisimulation on itrees. If [eq_itree RR t1 t2],
       we say that [t1] and [t2] are (strongly) bisimilar. As hinted
       at above, bisimilarity can be intuitively thought of as
       equality. *)
 
-  Definition eq_itree := eqit false false.
+  Definition eq_itree {R1 R2} := @eqit false false R1 R2.
 
-  Definition eutt := eqit true true.
+  Definition eutt {R1 R2} := @eqit true true R1 R2.
 
-  Definition euttge := eqit true false.
+  Definition euttge {R1 R2} := @eqit true false R1 R2.
+  
+End eqit_Definition.
 
-End eqit.
-
-(* begin hide *)
 Hint Constructors eqitF: core.
 Hint Unfold eqit_: core.
-Hint Resolve eqit__mono : paco.
-Hint Resolve eqit_idclo_mono : paco.
-Hint Unfold eqit: core.
+Hint Unfold eqiti : core.
+Hint Unfold eqitz : core.
+Hint Constructors eqit: core.
 Hint Unfold eq_itree: core.
 Hint Unfold eutt: core.
 Hint Unfold euttge: core.
 Hint Unfold id: core.
 
+Section eqit_Properties.
+
+  Context {E : Type -> Type}.
+
+  (** [eqitF] and [eqit_] are both monotone. *)
+
+  Lemma eqitF_mono R1 R2 RR RR' b1 b2 o o' x0 x1 sim sim'
+        (IN: @eqitF E b1 b2 R1 R2 RR sim o x0 x1)
+        (LER: RR <2= RR')
+        (LE: sim <3= sim')
+        (LEo: wfo_le o o'):
+    eqitF b1 b2 RR' sim' o' x0 x1.
+  Proof.
+    inv IN; eauto using wfo_lt_le_lt, wfo_le_le_le.
+    econstructor. intros. destruct (REL v). eauto.
+  Qed.
+
+  Lemma eqit__mono b1 b2: monotone6 (@eqit_ E b1 b2).
+  Proof.
+    red; intros. eapply eqitF_mono; eauto using wfo_le_refl.
+  Qed.
+
+End eqit_Properties.
+
+Hint Resolve eqit__mono : paco.
+
+(* begin hide *)
+
 Ltac unfold_eqit :=
-  (try match goal with [|- eqit_ _ _ _ _ _ _ _ ] => red end);
-  (repeat match goal with [H: eqit_ _ _ _ _ _ _ _ |- _ ] => red in H end).
+  (try match goal with [|- eqit_ _ _ _ _ _ _ _ _ _] => red end);
+  (repeat match goal with [H: eqit_ _ _ _ _ _ _ _ _ _|- _ ] => red in H end).
+
+Ltac fold_eqit :=
+  (try match goal with [|- eqitF ?b1 ?b2 ?RR (?sim _ _ _) ?o (observe ?t1) (observe ?t2)]
+                       => fold (eqit_ b1 b2 sim _ _ RR o t1 t2)
+       end);
+  (repeat match goal with [H: eqitF ?b1 ?b2 ?RR (?sim _ _ _) ?o (observe ?t1) (observe ?t2) |- _]
+                          => fold (eqit_ b1 b2 sim _ _ RR o t1 t2) in H
+          end).
 
 Lemma fold_eqitF:
-  forall {E R1 R2} (RR: R1 -> R2 -> Prop) b1 b2 (t1 : itree E R1) (t2 : itree E R2) ot1 ot2,
-    eqitF RR b1 b2 id (upaco2 (eqit_ RR b1 b2 id) bot2) ot1 ot2 ->
+  forall {E R1 R2} (RR: R1 -> R2 -> Prop) b1 b2 (t1 : itree E R1) (t2 : itree E R2) o ot1 ot2,
+    eqitF b1 b2 RR (upaco6 (eqit_ b1 b2) bot6 _ _ RR) o ot1 ot2 ->
     ot1 = observe t1 ->
     ot2 = observe t2 ->
-    eqit RR b1 b2 t1 t2.
+    eqit b1 b2 RR t1 t2.
 Proof.
-  intros * eq -> ->; pfold; auto.
+  intros * eq -> ->. eexists. pfold. eauto.
 Qed.
 
-Instance eqitF_Proper_R {E : Type -> Type} {R1 R2:Type} :
-  Proper ((@eq_rel R1 R2) ==> eq ==> eq ==> (eq_rel ==> eq_rel) ==> eq_rel ==> eq_rel)
-    (@eqitF E R1 R2).
+Definition eqit_rel_flip {E}
+           (r: forall R1 R2,(R1->R2->Prop)-> gwfo -> itree E R1 -> itree E R2 -> Prop)
+           R1 R2 RR o t1 t2 :=
+  r R2 R1 (flip RR) o t2 t1.
+
+Lemma eqitF_flip {E R1 R2} (RR : R1 -> R2 -> Prop) b1 b2 r:
+  (fun o => flip (eqitF b2 b1 (flip RR) (fun o => flip (r o)) o)) <3= @eqitF E b1 b2 R1 R2 RR r.
 Proof.
-  repeat red.
-  intros. subst. split; unfold subrelationH; intros.
-  - induction H0; try auto.
-    econstructor. apply H. assumption.
-    econstructor. apply H3. assumption.
-    econstructor. intros. specialize (REL v). specialize (H2 x3 y3). apply H2 in H3. apply H3. assumption.
-  - induction H0; try auto.
-    econstructor. apply H. assumption.
-    econstructor. apply H3. assumption.
-    econstructor. intros. specialize (REL v). specialize (H2 x3 y3). apply H2 in H3. apply H3. assumption.
+  intros. destruct PR; eauto.
 Qed.
 
-Instance eqitF_Proper_R2 {E : Type -> Type} {R1 R2:Type} :
-  Proper ((@eq_rel R1 R2) ==> eq ==> eq ==> eq ==> eq ==> eq ==> eq ==> iff)
-         (@eqitF E R1 R2).
+Lemma eqiti_r_flip E (r: forall R1 R2,(R1->R2->Prop)-> gwfo -> itree E R1 -> itree E R2 -> Prop) R1 R2 RR b1 b2
+      (u : itree E R1) (v : itree E R2) o
+      (REL: paco6 (eqit_ b2 b1) (eqit_rel_flip r) R2 R1 (flip RR) o v u)
+  : paco6 (eqit_ b1 b2) r R1 R2 RR o u v.
 Proof.
-  repeat red.
-  intros. subst. split; intros.
-  - induction H0; try auto.
-    econstructor. apply H. assumption.
-  - induction H0; try auto.
-    econstructor. apply H. assumption.
+  intros. revert_until b2. pcofix self. pstep; intros. punfold REL.
+  red. inv REL; econstructor; eauto; intros; edestruct REL0; eauto.
+  destruct H1; eauto.
 Qed.
 
-Instance eqit_Proper_R {E : Type -> Type} {R1 R2:Type}
-  : Proper ( (@eq_rel R1 R2) ==> eq ==> eq ==> eq ==> eq ==> iff) (@eqit E R1 R2).
+Lemma eqiti_flip E R1 R2 RR b1 b2:
+  forall (u : itree E R1) (v : itree E R2) o,
+    eqiti b2 b1 (flip RR) o v u -> eqiti b1 b2 RR o u v.
 Proof.
-  repeat red.
-  intros. subst.
-  split.
-  -  revert_until y1. pcofix CIH. intros.
-     pstep. punfold H1. red in H1. red.
-     hinduction H1 before CIH; intros; eauto.
-     + apply EqRet. apply H. assumption.
-     + apply EqTau. right. apply CIH. pclearbot. pinversion REL.
-     + apply EqVis. intros. red. right. apply CIH.
-       specialize (REL v).
-       red in REL. pclearbot. pinversion REL.
-  -  revert_until y1. pcofix CIH. intros.
-     pstep. punfold H1. red in H1. red.
-     hinduction H1 before CIH; intros; eauto.
-     + apply EqRet. apply H. assumption.
-     + apply EqTau. right. apply CIH. pclearbot. pinversion REL.
-     + apply EqVis. intros. red. right. apply CIH.
-       specialize (REL v).
-       red in REL. pclearbot. pinversion REL.
+  eauto using eqiti_r_flip.
 Qed.
 
-Instance eutt_Proper_R {E : Type -> Type} {R1 R2:Type}
-  : Proper ( (@eq_rel R1 R2) ==> eq ==> eq ==> iff) (@eutt E R1 R2).
-Proof.
-  unfold eutt. repeat red.
-  intros. split; intros; subst.
-  - rewrite <- H. assumption.
-  - rewrite H. assumption.
-Qed.
-
-
-Definition flip_clo {A B C} clo r := @flip A B C (clo (@flip B A C r)).
-
-Lemma eqitF_flip {E R1 R2} (RR : R1 -> R2 -> Prop) b1 b2 vclo r:
-  flip (eqitF (flip RR) b2 b1 (flip_clo vclo) (flip r)) <2= @eqitF E R1 R2 RR b1 b2 vclo r.
-Proof.
-  intros. induction PR; eauto.
-Qed.
-
-Lemma eqit_flip {E R1 R2} (RR : R1 -> R2 -> Prop) b1 b2:
+Lemma eqit_flip E R1 R2 RR b1 b2:
   forall (u : itree E R1) (v : itree E R2),
-    eqit (flip RR) b2 b1 v u -> eqit RR b1 b2 u v.
+    eqit b2 b1 (flip RR) v u -> eqit b1 b2 RR u v.
 Proof.
-  pcofix self; pstep. intros u v euv. punfold euv.
-  red in euv |- *. induction euv; pclearbot; eauto 7 with paco.
+  intros. destruct H. eauto using eqiti_flip.
 Qed.
 
-Lemma eqit_mon {E R1 R2} RR RR' (b1 b2 b1' b2': bool)
+Lemma eqiti_mon E R1 R2 RR RR' (b1 b2 b1' b2': bool) o o' t1 t2
+      (REL: @eqiti E b1 b2 R1 R2 RR o t1 t2)
+      (LEb1: b1 -> b1')
+      (LEb2: b2 -> b2')
+      (LEo: wfo_le o o')
+      (LERR: RR <2= RR'):
+  eqiti b1' b2' RR' o' t1 t2.
+Proof.
+  intros. revert o o' LEo t1 t2 REL. pcofix self. intros. pstep. punfold REL.
+  red. inv REL; pclearbot; econstructor; eauto using wfo_lt_le_lt, wfo_le_refl.
+  intros. destruct (REL0 v). pclearbot. eauto 7 using wfo_le_refl.
+Qed.
+
+Lemma eqit_mon E R1 R2 RR RR' (b1 b2 b1' b2': bool) t1 t2
+      (REL: @eqit E b1 b2 R1 R2 RR t1 t2)
       (LEb1: b1 -> b1')
       (LEb2: b2 -> b2')
       (LERR: RR <2= RR'):
-  @eqit E R1 R2 RR b1 b2 <2= eqit RR' b1' b2'.
+  eqit b1' b2' RR' t1 t2.
 Proof.
-  pcofix self. pstep. intros u v euv. punfold euv.
-  red in euv |- *. induction euv; pclearbot; eauto 7 with paco.
+  intros. destruct REL. exists o.
+  eapply eqiti_mon; eauto using wfo_le_refl.
 Qed.
 
 Hint Unfold flip: core.
+
+Instance eqitF_Proper_R {E : Type -> Type} b1 b2 {R1 R2:Type} :
+  Proper ((@eq_rel R1 R2) ==> (eq ==> eq_rel) ==> eq ==> eq_rel)
+    (@eqitF E b1 b2 R1 R2).
+Proof.
+  repeat red. intros. subst. split; red; intros.
+  - eapply eqitF_mono; intros; eauto using wfo_le_refl. eapply H; eauto. eapply H0; eauto.
+  - eapply eqitF_mono; intros; eauto using wfo_le_refl. eapply H; eauto. eapply H0; eauto.
+Qed.
+
+Instance eqitF_Proper_R2 {E : Type -> Type} b1 b2 {R1 R2:Type} :
+  Proper ((@eq_rel R1 R2) ==> eq ==> eq ==> eq ==> eq ==> iff)
+         (@eqitF E b1 b2 R1 R2).
+Proof.
+  repeat red. intros. subst. split; intros.
+  - eapply eqitF_mono; intros; eauto using wfo_le_refl. eapply H; eauto.
+  - eapply eqitF_mono; intros; eauto using wfo_le_refl. eapply H; eauto.
+Qed.
+        
+Instance eqit_Proper_R {E : Type -> Type} b1 b2 R1 R2
+  : Proper ((@eq_rel R1 R2) ==> eq ==> eq ==> iff) (@eqit E b1 b2 R1 R2).
+Proof.
+  unfold eq_rel. repeat red. intros. subst.
+  destruct H. unfold subrelationH in *.
+  eauto using eqit_mon.
+Qed.
+        
+Instance eutt_Proper_R {E : Type -> Type} {R1 R2:Type}
+  : Proper ( (@eq_rel R1 R2) ==> eq ==> eq ==> iff) (@eutt E R1 R2).
+Proof.
+  unfold eutt. repeat red. intros. subst.
+  destruct H. unfold subrelationH in *.
+  eauto using eqit_mon.
+Qed.
+
 
 (* end hide *)
 
@@ -279,112 +340,14 @@ Delimit Scope eq_itree_scope with eq_itree.
     tex-mode *)
 
 Open Scope itree.
-
+         
 Infix "≅" := (eq_itree eq) (at level 70) : itree_scope.
 
 Infix "≈" := (eutt eq) (at level 70) : itree_scope.
 
 Infix "≳" := (euttge eq) (at level 70) : itree_scope.
 
-Section eqit_closure.
-
-Context {E : Type -> Type} {R1 R2 : Type} (RR : R1 -> R2 -> Prop).
-
-(** *** "Up-to" principles for coinduction. *)
-
-Inductive eqit_trans_clo b1 b2 b1' b2' (r : itree E R1 -> itree E R2 -> Prop)
-  : itree E R1 -> itree E R2 -> Prop :=
-| eqit_trans_clo_intro t1 t2 t1' t2' RR1 RR2
-      (EQVl: eqit RR1 b1 b1' t1 t1')
-      (EQVr: eqit RR2 b2 b2' t2 t2')
-      (REL: r t1' t2')
-      (LERR1: forall x x' y, RR1 x x' -> RR x' y -> RR x y)
-      (LERR2: forall x y y', RR2 y y' -> RR x y' -> RR x y)
-  : eqit_trans_clo b1 b2 b1' b2' r t1 t2
-.
-Hint Constructors eqit_trans_clo: core.
-
-Definition eqitC b1 b2 := eqit_trans_clo b1 b2 false false.
-Hint Unfold eqitC: core.
-
-Lemma eqitC_mon b1 b2 r1 r2 t1 t2
-      (IN: eqitC b1 b2 r1 t1 t2)
-      (LE: r1 <2= r2):
-  eqitC b1 b2 r2 t1 t2.
-Proof.
-  destruct IN. econstructor; eauto.
-Qed.
-
-Hint Resolve eqitC_mon : paco.
-
-Lemma eqitC_wcompat b1 b2 vclo
-      (MON: monotone2 vclo)
-      (CMP: compose (eqitC b1 b2) vclo <3= compose vclo (eqitC b1 b2)):
-  wcompatible2 (@eqit_ E R1 R2 RR b1 b2 vclo) (eqitC b1 b2).
-Proof.
-  econstructor. pmonauto.
-  intros. dependent destruction PR.
-  punfold EQVl. punfold EQVr. unfold_eqit.
-  hinduction REL before r; intros; clear t1' t2'.
-  - remember (RetF r1) as x.
-    hinduction EQVl before r; intros; subst; try inv Heqx; eauto.
-    remember (RetF r3) as y.
-    hinduction EQVr before r; intros; subst; try inv Heqy; eauto.
-  - remember (TauF m1) as x.
-    hinduction EQVl before r; intros; subst; try inv Heqx; try inv CHECK; eauto.
-    remember (TauF m3) as y.
-    hinduction EQVr before r; intros; subst; try inv Heqy; try inv CHECK; eauto.
-    pclearbot. econstructor. gclo.
-    econstructor; cycle -1; eauto with paco.
-  - remember (VisF e k1) as x.
-    hinduction EQVl before r; intros; subst; try dependent destruction Heqx; try inv CHECK; eauto.
-    remember (VisF e0 k3) as y.
-    hinduction EQVr before r; intros; subst; try dependent destruction Heqy; try inv CHECK; eauto.
-    econstructor. intros. pclearbot.
-    eapply MON.
-    + apply CMP. econstructor; eauto.
-    + intros. apply gpaco2_clo, PR.
-  - remember (TauF t1) as x.
-    hinduction EQVl before r; intros; subst; try inv Heqx; try inv CHECK; eauto.
-    pclearbot. punfold REL.
-  - remember (TauF t2) as y.
-    hinduction EQVr before r; intros; subst; try inv Heqy; try inv CHECK; eauto.
-    pclearbot. punfold REL.
-Qed.
-
-Hint Resolve eqitC_wcompat : paco.
-
-Lemma eqit_idclo_compat b1 b2: compose (eqitC b1 b2) id <3= compose id (eqitC b1 b2).
-Proof.
-  intros. apply PR.
-Qed.
-Hint Resolve eqit_idclo_compat : paco.
-
-Lemma eqitC_dist b1 b2:
-  forall r1 r2, eqitC b1 b2 (r1 \2/ r2) <2= (eqitC b1 b2 r1 \2/ eqitC b1 b2 r2).
-Proof.
-  intros. destruct PR. destruct REL; eauto.
-Qed.
-
-Hint Resolve eqitC_dist : paco.
-
-Lemma eqit_clo_trans b1 b2 vclo
-      (MON: monotone2 vclo)
-      (CMP: compose (eqitC b1 b2) vclo <3= compose vclo (eqitC b1 b2)):
-  eqit_trans_clo b1 b2 false false <3= gupaco2 (eqit_ RR b1 b2 vclo) (eqitC b1 b2).
-Proof.
-  intros. destruct PR. gclo. econstructor; eauto with paco.
-Qed.
-
-End eqit_closure.
-
-Hint Unfold eqitC: core.
-Hint Resolve eqitC_mon : paco.
-Hint Resolve eqitC_wcompat : paco.
-Hint Resolve eqit_idclo_compat : paco.
-Hint Resolve eqitC_dist : paco.
-Arguments eqit_clo_trans : clear implicits.
-Hint Constructors eqit_trans_clo: core.
+Hint Resolve cpn6_wcompat : core.
 
 (** ** Properties of relations *)
 
@@ -394,146 +357,225 @@ Section eqit_gen.
 
 (** *** Properties of relation transformers. *)
 
-Context {E : Type -> Type} {R: Type} (RR : R -> R -> Prop).
+Context {E : Type -> Type}.
 
-Global Instance Reflexive_eqitF b1 b2 (sim : itree E R -> itree E R -> Prop)
-: Reflexive RR -> Reflexive sim -> Reflexive (eqitF RR b1 b2 id sim).
+Global Instance Reflexive_eqitF b1 b2 {R: Type} (RR : R -> R -> Prop) sim
+  : Reflexive RR -> (forall o, Reflexive (sim o)) ->
+    forall o, Reflexive (@eqitF E b1 b2 _ _ RR sim o).
 Proof.
-  red. destruct x; constructor; eauto.
+  red; intros. red in H0. destruct x; eauto using wfo_le_refl.
+  Grab Existential Variables. eauto.
 Qed.
 
-Global Instance Symmetric_eqitF b (sim : itree E R -> itree E R -> Prop)
-: Symmetric RR -> Symmetric sim -> Symmetric (eqitF RR b b id sim).
+Global Instance Symmetric_eqitF b {R: Type} (RR : R -> R -> Prop) sim
+  : Symmetric RR -> (forall o, Symmetric (sim o)) ->
+    forall o, Symmetric (@eqitF E b b _ _ RR sim o).
 Proof.
-  red. induction 3; constructor; subst; eauto.
-  intros. apply H0. apply (REL v).
+  red; intros. red in H0. dependent destruction H1; eauto.
+  econstructor. intros. destruct (REL v). eauto.
 Qed.
 
-Global Instance Reflexive_eqit_ b1 b2 (sim : itree E R -> itree E R -> Prop)
-: Reflexive RR -> Reflexive sim -> Reflexive (eqit_ RR b1 b2 id sim).
-Proof. repeat red. intros. reflexivity. Qed.
+Global Instance Reflexive_eqit_ b1 b2 R (RR: R->R->Prop) (sim: forall R1 R2,(R1->R2->Prop)->_->_->_->Prop)
+  : Reflexive RR ->
+    (forall o, Reflexive (sim R R RR o)) ->
+    forall o, Reflexive (@eqit_ E b1 b2 sim R R RR o).
+Proof.
+  red. intros. eapply Reflexive_eqitF; eauto.
+Qed.
 
-Global Instance Symmetric_eqit_ b (sim : itree E R -> itree E R -> Prop)
-: Symmetric RR -> Symmetric sim -> Symmetric (eqit_ RR b b id sim).
-Proof. repeat red; symmetry; auto. Qed.
+Global Instance Symmetric_eqit_ b R (RR: R->R->Prop) (sim: forall R1 R2,(R1->R2->Prop)->_->_->_->Prop)
+  : Symmetric RR ->
+    (forall o,  Symmetric (sim R R RR o)) ->
+    forall o, Symmetric (@eqit_ E b b sim R R RR o).
+Proof.
+  red. intros. eapply Symmetric_eqitF; eauto.
+Qed.
 
 (** *** [eqit] is an equivalence relation *)
 
-Global Instance Reflexive_eqit_gen b1 b2 (r rg: itree E R -> itree E R -> Prop) :
-  Reflexive RR -> Reflexive (gpaco2 (eqit_ RR b1 b2 id) (eqitC RR b1 b2) r rg).
+Global Instance Reflexive_eqit_gen b1 b2 r rg R (RR:R->R->Prop) o
+  : Reflexive RR ->
+    Reflexive (gpaco6 (@eqit_ E b1 b2) (cpn6 (eqit_ b1 b2)) r rg R R RR o).
 Proof.
   gcofix CIH. gstep; intros.
-  repeat red. destruct (observe x); eauto with paco.
+  repeat red. destruct (observe x); eauto using wfo_le_refl with paco.
 Qed.
 
-Global Instance Reflexive_eqit b1 b2 : Reflexive RR -> Reflexive (@eqit E _ _ RR b1 b2).
+Global Instance Reflexive_eqiti b1 b2 R (RR:R->R->Prop) o
+  : Reflexive RR -> Reflexive (@eqiti E b1 b2 R R RR o).
 Proof.
-  red; intros. ginit. apply Reflexive_eqit_gen; eauto.
+  ginit. intros. apply Reflexive_eqit_gen; eauto.
 Qed.
 
-Global Instance Symmetric_eqit b : Symmetric RR -> Symmetric (@eqit E _ _ RR b b).
+Global Instance Reflexive_eqit b1 b2 R (RR:R->R->Prop)
+  : Reflexive RR -> Reflexive (@eqit E b1 b2 R R RR).
 Proof.
-  red; intros. apply eqit_flip.
-  eapply eqit_mon, H0; eauto.
+  econstructor. apply Reflexive_eqiti. eauto.
+  Grab Existential Variables. eapply wfo_zero.
 Qed.
 
-Global Instance eq_sub_euttge:
-  subrelation (@eq_itree E _ _ RR) (euttge RR).
+Global Instance Symmetric_eqiti b R (RR:R->R->Prop) o
+  : Symmetric RR -> Symmetric (@eqiti E b b R R RR o).
 Proof.
-  ginit. gcofix CIH. intros.
-  punfold H0. gstep. red in H0 |- *.
-  hinduction H0 before CIH; subst; econstructor; try inv CHECK; pclearbot; eauto 7 with paco.
+  red; intros. apply eqiti_flip.
+  eapply eqiti_mon; eauto using wfo_le_refl.
 Qed.
 
-Global Instance euttge_sub_eutt:
-  subrelation (@euttge E _ _ RR) (eutt RR).
+Global Instance Symmetric_eqit b R (RR:R->R->Prop)
+  : Symmetric RR -> Symmetric (@eqit E b b R R RR).
 Proof.
-  ginit. gcofix CIH. intros.
-  punfold H0. gstep. red in H0 |- *.
-  hinduction H0 before CIH; subst; econstructor; pclearbot; eauto 7 with paco.
+  red. intros. destruct H0. exists o.
+  apply Symmetric_eqiti; eauto.
 Qed.
 
-Global Instance eq_sub_eutt:
-  subrelation (@eq_itree E _ _ RR) (eutt RR).
+Global Instance eq_sub_euttge R RR
+  : subrelation (@eq_itree E R R RR) (euttge RR).
+Proof.
+  red; intros. destruct H. exists o.
+  ginit. revert_until E.
+  gcofix CIH. intros.
+  punfold REL. gstep.
+  red in REL |- *.
+  inv REL; pclearbot; eauto 7 with paco.
+  econstructor. intros. destruct (REL0 v). pclearbot. eauto with paco.
+Qed.
+
+Global Instance euttge_sub_eutt R RR
+  : subrelation (@euttge E R R RR) (eutt RR).
+Proof.
+  red; intros. destruct H. exists o.
+  ginit. revert_until E.
+  gcofix CIH. intros.
+  punfold REL. gstep.
+  red in REL |- *.
+  inv REL; pclearbot; eauto 7 with paco.
+  econstructor. intros. destruct (REL0 v). pclearbot. eauto with paco.
+Qed.
+
+Global Instance eq_sub_eutt R RR
+  : subrelation (@eq_itree E R R RR) (eutt RR).
 Proof.
   red; intros. eapply euttge_sub_eutt. eapply eq_sub_euttge. apply H.
 Qed.
 
 End eqit_gen.
 
-Hint Resolve Reflexive_eqit Reflexive_eqit_gen : reflexivity.
+Hint Resolve Reflexive_eqit Reflexive_eqiti Reflexive_eqit_gen : reflexivity.
 
 Section eqit_eq.
 
 (** *** Properties of relation transformers. *)
 
-Context {E : Type -> Type} {R : Type}.
+Context {E : Type -> Type} {R: Type}.
 
-Local Notation eqit := (@eqit E R R eq).
-
-Global Instance Reflexive_eqitF_eq b1 b2 (sim : itree E R -> itree E R -> Prop)
-: Reflexive sim -> Reflexive (eqitF eq b1 b2 id sim).
+Global Instance Reflexive_eqitF_eq b1 b2 sim
+  : (forall o, Reflexive (sim o)) ->
+    forall o, Reflexive (@eqitF E b1 b2 R R eq sim o).
 Proof.
   apply Reflexive_eqitF; eauto.
 Qed.
 
-Global Instance Symmetric_eqitF_eq b (sim : itree E R -> itree E R -> Prop)
-: Symmetric sim -> Symmetric (eqitF eq b b id sim).
+Global Instance Symmetric_eqitF_eq b sim
+  : (forall o, Symmetric (sim o)) ->
+    forall o, Symmetric (@eqitF E b b R R eq sim o).
 Proof.
   apply Symmetric_eqitF; eauto.
 Qed.
 
-Global Instance Reflexive_eqit__eq b1 b2 (sim : itree E R -> itree E R -> Prop)
-: Reflexive sim -> Reflexive (eqit_ eq b1 b2 id sim).
-Proof. apply Reflexive_eqit_; eauto. Qed.
+Global Instance Reflexive_eqit__eq b1 b2 (sim: forall R1 R2,(R1->R2->Prop)->_->_->_->_)
+  : (forall o, Reflexive (sim R R eq o)) ->
+    forall o, Reflexive (@eqit_ E b1 b2 sim R R eq o).
+Proof. intros. eapply Reflexive_eqit_; eauto. Qed.
 
-Global Instance Symmetric_eqit__eq b (sim : itree E R -> itree E R -> Prop)
-: Symmetric sim -> Symmetric (eqit_ eq b b id sim).
+Global Instance Symmetric_eqit__eq b (sim: forall R1 R2,(R1->R2->Prop)->_->_->_->_)
+  : (forall o, Symmetric (sim R R eq o)) ->
+    forall o, Symmetric (@eqit_ E b b sim R R eq o).
 Proof. apply Symmetric_eqit_; eauto. Qed.
 
 (** *** [eqit] is an equivalence relation *)
 
-Global Instance Reflexive_eqit_gen_eq b1 b2 (r rg: itree E R -> itree E R -> Prop) :
-  Reflexive (gpaco2 (eqit_ eq b1 b2 id) (eqitC eq b1 b2) r rg).
+Global Instance Reflexive_eqit_gen_eq b1 b2 r rg
+  : forall o, Reflexive (gpaco6 (@eqit_ E b1 b2) (cpn6 (eqit_ b1 b2)) r rg R R eq o).
 Proof.
-  apply Reflexive_eqit_gen; eauto.
+  intros. apply Reflexive_eqit_gen; eauto.
 Qed.
 
-Global Instance Reflexive_eqit_eq b1 b2 : Reflexive (eqit b1 b2).
+Global Instance Reflexive_eqiti_eq b1 b2 o
+  : Reflexive (@eqiti E b1 b2 R R eq o).
+Proof.
+  apply Reflexive_eqiti; eauto.
+Qed.
+
+Global Instance Reflexive_eqit_eq b1 b2
+  : Reflexive (@eqit E b1 b2 R R eq).
 Proof.
   apply Reflexive_eqit; eauto.
 Qed.
 
-Global Instance Symmetric_eqit_eq b : Symmetric (eqit b b).
+Global Instance Symmetric_eqiti_eq b o
+  : Symmetric (@eqiti E b b R R eq o).
+Proof.
+  apply Symmetric_eqiti; eauto.
+Qed.
+
+Global Instance Symmetric_eqit_eq b
+  : Symmetric (@eqit E b b R R eq).
 Proof.
   apply Symmetric_eqit; eauto.
 Qed.
 
 (** *** Congruence properties *)
 
-Global Instance eqit_observe b1 b2:
-  Proper (eqit b1 b2 ==> going (eqit b1 b2)) (@observe E R).
+Global Instance eqiti_observe b1 b2 o:
+  Proper (eqiti b1 b2 eq o ==> going (eqiti b1 b2 eq o)) (@observe E R).
 Proof.
-  constructor; punfold H.
+  constructor. punfold H.
+Qed.
+
+Global Instance eqit_observe b1 b2:
+  Proper (eqit b1 b2 eq ==> going (eqit b1 b2 eq)) (@observe E R).
+Proof.
+  constructor. destruct H. exists o. punfold REL.
+Qed.
+
+Global Instance eqiti_tauF b1 b2 o:
+  Proper (eqiti b1 b2 eq o ==> going (eqiti b1 b2 eq o)) (@TauF E R _).
+Proof.
+  constructor. pstep. econstructor; eauto using wfo_le_refl.
 Qed.
 
 Global Instance eqit_tauF b1 b2:
-  Proper (eqit b1 b2 ==> going (eqit b1 b2)) (@TauF E R _).
+  Proper (eqit b1 b2 eq ==> going (eqit b1 b2 eq)) (@TauF E R _).
 Proof.
-  constructor; pstep. econstructor. eauto.
+  constructor. destruct H. exists o. pstep. econstructor; eauto using wfo_le_refl.
 Qed.
 
-Global Instance eqit_VisF b1 b2 {u} (e: E u) :
-  Proper (pointwise_relation _ (eqit b1 b2) ==> going (eqit b1 b2)) (VisF e).
+Global Instance eqiti_visF b1 b2 o {u} (e: E u):
+  Proper (pointwise_relation _ (eqiti b1 b2 (@eq R) o) ==> going (eqiti b1 b2 eq o)) (VisF e).
 Proof.
-  constructor; red in H. unfold eqit in *. pstep; econstructor; eauto.
+  econstructor. pstep.
+  econstructor. intros. specialize (H v). eauto.
 Qed.
 
-Global Instance observing_sub_eqit l r :
-  subrelation (observing eq) (eqit l r).
+Global Instance eqit_visF b1 b2 {u} (e: E u) :
+  Proper (pointwise_relation _ (eqit b1 b2 (@eq R)) ==> going (eqit b1 b2 eq)) (VisF e).
 Proof.
-  repeat red; intros. destruct H.
-  pstep. red. rewrite H. apply Reflexive_eqitF; eauto. left. apply reflexivity.
+  econstructor. exists wfo_zero. pstep.
+  econstructor. intros. destruct (H v). eauto.
+Qed.
+
+Global Instance observing_sub_eqiti b1 b2 o :
+  subrelation (observing eq) (@eqiti E b1 b2 R R eq o).
+Proof.
+  repeat red; intros. pstep. red. rewrite H.
+  apply Reflexive_eqitF; eauto.
+  intros. left. apply Reflexive_eqiti. eauto.
+Qed.
+
+Global Instance observing_sub_eqit b1 b2 :
+  subrelation (observing eq) (@eqit E b1 b2 R R eq).
+Proof.
+  exists wfo_zero. eapply observing_sub_eqiti. eauto.
 Qed.
 
 (** ** Eta-expansion *)
@@ -551,166 +593,229 @@ End eqit_eq.
 Lemma eq_itree_inv_ret {E R} (t : itree E R) r :
   t ≅ (Ret r) -> observe t = RetF r.
 Proof.
-  intros; punfold H; inv H; try inv CHECK; eauto.
+  intros. destruct H. punfold REL. inv REL; try inv CHECK; try inv CHECK1; try inv CHECK2; eauto.
 Qed.
 
 Lemma eq_itree_inv_vis {E R U} (t : itree E R) (e : E U) (k : U -> _) :
   t ≅ Vis e k -> exists k', observe t = VisF e k' /\ forall u, k' u ≅ k u.
 Proof.
-  intros; punfold H; inv H; auto_inj_pair2; subst; try inv CHECK.
+  intros. destruct H. punfold REL; inv REL; auto_inj_pair2; subst; try inv CHECK; try inv CHECK1; try inv CHECK2.
   eexists; split; eauto.
-  intros. destruct (REL u); try contradiction; pclearbot; eauto.
+  intros. destruct (REL0 u); try contradiction; pclearbot; eauto.
 Qed.
 
 Lemma eq_itree_inv_tau {E R} (t t' : itree E R) :
   t ≅ Tau t' -> exists t0, observe t = TauF t0 /\ t0 ≅ t'.
 Proof.
-  intros; punfold H; inv H; try inv CHECK; pclearbot; eauto.
+  intros; destruct H. punfold REL; inv REL; try inv CHECK; try inv CHECK1; try inv CHECK2; pclearbot; eauto.
 Qed.
 
 Lemma eqit_inv_ret {E R1 R2 RR} b1 b2 r1 r2 :
-  @eqit E R1 R2 RR b1 b2 (Ret r1) (Ret r2) -> RR r1 r2.
+  @eqit E b1 b2 R1 R2 RR (Ret r1) (Ret r2) -> RR r1 r2.
 Proof.
-  intros. punfold H. inv H. eauto.
+  intros. destruct H as [? H].
+  assert (WFo := wfo_wf _ o). induction WFo.
+  punfold H. inv H; eauto.
+  eapply H1; eauto.
+  pclearbot. rewrite <-H3, <-H4. punfold REL.
 Qed.
 
 Lemma eqit_inv_vis {E R1 R2 RR} b1 b2 {u} (e1 e2: E u) (k1: u -> itree E R1) (k2: u -> itree E R2) :
-  eqit RR b1 b2 (Vis e1 k1) (Vis e2 k2) -> e1 = e2 /\ (forall u, eqit RR b1 b2 (k1 u) (k2 u)).
+  eqit b1 b2 RR (Vis e1 k1) (Vis e2 k2) -> e1 = e2 /\ (forall u, eqit b1 b2 RR (k1 u) (k2 u)).
 Proof.
-  intros. punfold H. repeat red in H. simpl in H.
-  dependent destruction H. pclearbot. eauto.
+  intros. destruct H as [? H].
+  assert (WFo := wfo_wf _ o). induction WFo.
+  punfold H. repeat red in H. simpl in H.
+  dependent destruction H.
+  - split; eauto. intros y. destruct (REL y). pclearbot. eauto.
+  - eapply H1; eauto.
+    pclearbot. rewrite <-x1, <-x. punfold REL.
 Qed.
 
-Lemma eqit_inv_tauL {E R1 R2 RR} b1 t1 t2 :
-  @eqit E R1 R2 RR b1 true (Tau t1) t2 -> eqit RR b1 true t1 t2.
+Lemma eqiti_inv_tauL E b1 R1 R2 RR o o' t1 t2
+      (REL: @eqiti E b1 true R1 R2 RR o (Tau t1) t2)
+      (LT: wfo_lt o o')
+  : eqiti b1 true RR o' t1 t2.
 Proof.
-  intros. punfold H. red in H. simpl in *.
-  remember (TauF t1) as tt1. genobs t2 ot2.
-  hinduction H before b1; intros; try discriminate.
-  - inv Heqtt1. pclearbot. pstep. red. simpobs. econstructor; eauto. pstep_reverse.
-  - inv Heqtt1. punfold_reverse H.
-  - red in IHeqitF. pstep. red; simpobs. econstructor; eauto. pstep_reverse.
+  revert_until RR. pcofix CIH. intros.
+  revert_until o. assert (WF := wfo_wf _ o). induction WF; intros.
+  pfold. punfold REL. red in REL |- *. inv REL.
+  - econstructor; eauto.
+    pclearbot. left. eapply paco6_mon_bot; eauto.
+    eapply eqiti_mon; eauto.
+  - pclearbot. punfold REL0.
+    eapply eqitF_mono; eauto using wfo_lt_le, wfo_le_le_le, upaco6_mon_bot.
+  - econstructor; eauto.
+    right. eapply CIH; eauto.
+    pclearbot. punfold REL0. pfold. rewrite <- H2. eauto.
+  - econstructor; eauto.
+    right. eapply CIH; eauto.
+    pclearbot. punfold REL0. pfold. rewrite <- H2. eauto.
 Qed.
 
-Lemma eqit_inv_tauR {E R1 R2 RR} b2 t1 t2 :
-  @eqit E R1 R2 RR true b2 t1 (Tau t2) -> eqit RR true b2 t1 t2.
+Lemma eqiti_inv_tauR E b2 R1 R2 RR o o' t1 t2
+      (REL: @eqiti E true b2 R1 R2 RR o t1 (Tau t2))      
+      (LT: wfo_lt o o')
+  : eqiti true b2 RR o' t1 t2.
 Proof.
-  intros. punfold H. red in H. simpl in *.
-  remember (TauF t2) as tt2. genobs t1 ot1.
-  hinduction H before b2; intros; try discriminate.
-  - inv Heqtt2. pclearbot. pstep. red. simpobs. econstructor; eauto. pstep_reverse.
-  - red in IHeqitF. pstep. red; simpobs. econstructor; eauto. pstep_reverse.
-  - inv Heqtt2. punfold_reverse H.
+  revert_until RR. pcofix CIH. intros.
+  revert_until o. assert (WF := wfo_wf _ o). induction WF; intros.
+  pfold. punfold REL. red in REL |- *. inv REL.
+  - econstructor; eauto.
+    pclearbot. left. eapply paco6_mon_bot; eauto.
+    eapply eqiti_mon; eauto.
+  - econstructor; eauto.
+    right. eapply CIH; eauto.
+    pclearbot. punfold REL0. pfold. rewrite <- H3. eauto.
+  - pclearbot. punfold REL0.
+    eapply eqitF_mono; eauto using wfo_lt_le, wfo_le_le_le, upaco6_mon_bot.
+  - econstructor; eauto.
+    right. eapply CIH; eauto.
+    pclearbot. punfold REL0. pfold. rewrite <- H3. eauto.
 Qed.
 
-Lemma eqit_inv_tauLR {E R1 R2 RR} b1 b2 t1 t2 :
-  @eqit E R1 R2 RR b1 b2 (Tau t1) (Tau t2) -> eqit RR b1 b2 t1 t2.
+Lemma eqiti_inv_tauLR E b1 b2 R1 R2 RR o t1 t2
+      (REL: @eqiti E b1 b2 R1 R2 RR o (Tau t1) (Tau t2))
+  : eqiti b1 b2 RR o t1 t2.
 Proof.
-  intros. punfold H. red in H. simpl in *.
-  remember (TauF t1) as tt1. remember (TauF t2) as tt2.
-  hinduction H before b2; intros; try discriminate.
-  - inv Heqtt1. inv Heqtt2. pclearbot. eauto.
-  - inv Heqtt1. inv H; eauto.
-    + pclearbot. punfold REL. pstep. red. simpobs. eauto.
-    + pstep. red. simpobs. econstructor; eauto. pstep_reverse. apply IHeqitF; eauto.
-  - inv Heqtt2. inv H; eauto.
-    + pclearbot. punfold REL. pstep. red. simpobs. eauto.
-    + pstep. red. simpobs. econstructor; eauto. pstep_reverse. apply IHeqitF; eauto.
+  revert_until o. assert (WF := wfo_wf _ o). induction WF as [o _ HYP]; intros.
+  punfold REL. red in REL. inv REL; pclearbot; subst.
+  - eauto using eqiti_mon.
+  - destruct b1; inv CHECK.
+    eapply eqiti_inv_tauR; eauto.
+    punfold REL0. pfold. red. rewrite <-H. eauto.
+  - destruct b2; inv CHECK.
+    eapply eqiti_inv_tauL; eauto.
+    punfold REL0. pfold. red. rewrite <-H0. eauto.
+  - pstep. econstructor; eauto.
+    left. eapply HYP; eauto.
+    rewrite <-H,<-H0. pstep. punfold REL0.
 Qed.
 
 Lemma eqit_inv_ret_vis: forall {E X R1 R2 RR} b1 b2 (r: R1) (e: E X) k,
-    @eqit E R1 R2 RR b1 b2 (Ret r) (Vis e k) -> False.
+    @eqit E b1 b2 R1 R2 RR (Ret r) (Vis e k) -> False.
 Proof.
-  intros.
+  intros. destruct H as [? H].
+  assert (WF := wfo_wf _ o). induction WF as [o _ HYP]; intros.
   punfold H; inv H.
+  eapply HYP; eauto.
+  rewrite <-H1, <-H2. pclearbot. pstep. punfold REL.
 Qed.
 
 Lemma eutt_inv_ret_vis: forall {X Y E} (x: X) (e: E Y) k, Ret x ≈ Vis e k -> False.
 Proof.
-  intros; eapply eqit_inv_ret_vis; eauto.
+  intros. destruct H. eapply eqit_inv_ret_vis; eauto.
 Qed.
 
 Lemma eqitree_inv_ret_vis: forall {X Y E} (x: X) (e: E Y) k, Ret x ≅ Vis e k -> False.
 Proof.
-  intros; eapply eqit_inv_ret_vis; eauto.
+  intros. destruct H. eapply eqit_inv_ret_vis; eauto.
 Qed.
 
 Lemma eqit_inv_tau_vis: forall {E X R1 R2 RR} b2 (e: E X) k t,
-    @eqit E R1 R2 RR false b2 (Tau t) (Vis e k) -> False.
+    @eqit E false b2 R1 R2 RR (Tau t) (Vis e k) -> False.
 Proof.
-  intros.
+  intros. destruct H as [? H].
   punfold H; inv H.
-  inv CHECK.
+  inv CHECK. inv CHECK1.
 Qed.
 
 Lemma eqit_inv_vis_tau: forall {E X R1 R2 RR} b1 (e: E X) k t,
-    @eqit E R1 R2 RR b1 false (Vis e k) (Tau t) -> False.
+    @eqit E b1 false R1 R2 RR (Vis e k) (Tau t) -> False.
 Proof.
-  intros.
+  intros. destruct H as [? H].
   punfold H; inv H.
-  inv CHECK.
+  inv CHECK. inv CHECK2.
 Qed.
 
 Lemma euttge_inv_tau_vis: forall {E A B} (e: E A) (k : A -> itree E B) (a : itree E B), Vis e k ≳ Tau a -> False.
 Proof.
-  intros; eapply eqit_inv_vis_tau; eauto.
+  intros. destruct H. eapply eqit_inv_vis_tau; eauto.
 Qed.
 
 Lemma eqitree_inv_tau_vis: forall {E A B} (e: E A) (k : A -> itree E B) (a : itree E B), Tau a ≅ Vis e k -> False.
 Proof.
-  intros; eapply eqit_inv_tau_vis; eauto.
+  intros. destruct H. eapply eqit_inv_tau_vis; eauto.
 Qed.
 
 Lemma eqit_inv_ret_tau: forall {E R1 R2 RR} b1 (r: R1) t,
-    @eqit E R1 R2 RR b1 false (Ret r) (Tau t) -> False.
+    @eqit E b1 false R1 R2 RR (Ret r) (Tau t) -> False.
 Proof.
-  intros.
+  intros. destruct H as [? H].
   punfold H; inv H.
-  inv CHECK.
+  inv CHECK. inv CHECK2.
 Qed.
 
 Lemma eqit_inv_tau_ret: forall {E R1 R2 RR} b2 (r: R2) t,
-    @eqit E R1 R2 RR false b2 (Tau t) (Ret r) -> False.
+    @eqit E false b2 R1 R2 RR (Tau t) (Ret r) -> False.
 Proof.
-  intros.
+  intros. destruct H as [? H].
   punfold H; inv H.
-  inv CHECK.
+  inv CHECK. inv CHECK1.
 Qed.
 
 Lemma euttge_inv_ret_tau: forall {E A} (r : A) (a : itree E A),
     Ret r ≳ Tau a -> False.
 Proof.
-  intros; eapply eqit_inv_ret_tau; eauto.
+  intros. destruct H. eapply eqit_inv_ret_tau; eauto.
 Qed.
 
 Lemma eqitree_inv_ret_tau: forall {E A} (r : A) (a : itree E A),
     Ret r ≅ Tau a -> False.
 Proof.
-  intros; eapply eqit_inv_ret_tau; eauto.
+  intros. destruct H. eapply eqit_inv_ret_tau; eauto.
 Qed.
 
 Lemma eutt_inv_ret {E R} r1 r2 :
   (Ret r1: itree E R) ≈ (Ret r2) -> r1 = r2.
 Proof.
-  intros; eapply eqit_inv_ret; eauto.
+  intros. destruct H. eapply eqit_inv_ret; eauto.
 Qed.
 
 Lemma eqitree_inv_ret {E R} r1 r2 :
   (Ret r1: itree E R) ≅ (Ret r2) -> r1 = r2.
 Proof.
-  intros; eapply eqit_inv_ret; eauto.
+  intros. destruct H. eapply eqit_inv_ret; eauto.
 Qed.
 
+(** [eqit] is a congruence for [itree] constructors. *)
+
 Lemma eqit_tauL {E R1 R2 RR} b2 (t1 : itree E R1) (t2 : itree E R2) :
-  eqit RR true b2 t1 t2 -> eqit RR true b2 (Tau t1) t2.
+  eqit true b2 RR t1 t2 -> eqit true b2 RR (Tau t1) t2.
 Proof.
-  intros. pstep. econstructor; eauto. punfold H.
+  intros. destruct H as [? H]. eexists. pstep. econstructor; eauto using wfo_add_one.
 Qed.
 
 Lemma eqit_tauR {E R1 R2 RR} b1 (t1 : itree E R1) (t2 : itree E R2) :
-  eqit RR b1 true t1 t2 -> eqit RR b1 true t1 (Tau t2).
+  eqit b1 true RR t1 t2 -> eqit b1 true RR t1 (Tau t2).
 Proof.
-  intros. pstep. econstructor; eauto. punfold H.
+  intros. destruct H as [? H]. eexists. pstep. econstructor; eauto using wfo_add_one.
+Qed.
+
+Lemma eqit_tau {E R1 R2 RR} b1 b2 (t1 : itree E R1) (t2 : itree E R2) :
+  eqit b1 b2 RR (Tau t1) (Tau t2) <-> eqit b1 b2 RR t1 t2.
+Proof.
+  split; intros [].
+  - eexists. eapply eqiti_inv_tauLR. eauto.
+  - eexists. pstep. econstructor; eauto using wfo_le_refl.
+Qed.
+
+Lemma eqit_vis {E R1 R2 RR} b1 b2 {U} (e : E U)
+      (k1 : U -> itree E R1) (k2 : U -> itree E R2) :
+      (forall u, eqit b1 b2 RR (k1 u) (k2 u))
+  <-> eqit b1 b2 RR (Vis e k1) (Vis e k2).
+Proof.
+  split; intros.
+  - exists wfo_zero. pstep. econstructor. intros. destruct (H v). eauto.
+  - eapply eqit_inv_vis; eauto.
+Qed.
+
+Lemma eqit_ret {E R1 R2 RR} b1 b2 (r1 : R1) (r2 : R2) :
+  RR r1 r2 <-> @eqit E b1 b2 _ _ RR (Ret r1) (Ret r2).
+Proof.
+  split; intros H.
+  - exists wfo_zero. pstep. constructor; auto.
+  - eapply eqit_inv_ret; eauto.
 Qed.
 
 Lemma tau_euttge {E R} (t: itree E R) :
@@ -727,87 +832,628 @@ Qed.
 
 Lemma simpobs {E R} {ot} {t: itree E R} (EQ: ot = observe t): t ≅ go ot.
 Proof.
-  pstep. repeat red. simpobs. simpl. subst. pstep_reverse. apply Reflexive_eqit; eauto.
+  exists wfo_zero. pstep.
+  unfold_eqit. simpobs. simpl. subst. fold_eqit.
+  pstep_reverse. eapply Reflexive_eqiti; eauto.
+Qed.
+
+(*************************)
+(** *** Eqit Lower Order *)
+(*************************)
+
+Variant euttOrdF (euttOrd : Type) :=
+| OBaseF
+| OTauF (o : euttOrd)
+| OStepF (o : euttOrd)
+.
+Arguments OBaseF {euttOrd}.
+Arguments OStepF {euttOrd} o.
+Arguments OTauF {euttOrd} o.
+
+CoInductive euttOrd : Type := ord_go
+{ ord_observe : euttOrdF euttOrd }.
+
+Notation euttOrd' := (euttOrdF euttOrd).
+Notation OBase := {| ord_observe := OBaseF |}.
+Notation OTau o := {| ord_observe := OTauF o |}.
+Notation OStep o := {| ord_observe := OStepF o |}.
+
+Inductive euttOrd_le': euttOrd' -> euttOrd' -> Prop :=
+| euttOrd_le_refl
+    o
+  : euttOrd_le' o o
+| euttOrd_le_step
+    o1 o2
+    (REL: euttOrd_le' o1 (ord_observe o2))
+  : euttOrd_le' o1 (OStepF o2)
+| euttOrd_le_tau
+    o1 o2
+    (REL: euttOrd_le' o1 (ord_observe o2))
+  : euttOrd_le' o1 (OTauF o2)
+.
+Hint Constructors euttOrd_le'.
+
+Definition euttOrd_le o1 o2 := euttOrd_le' (ord_observe o1) (ord_observe o2).
+Hint Unfold euttOrd_le.
+
+Inductive euttOrd_lt': euttOrd' -> euttOrd' -> Prop :=
+| euttOrd_lt_step
+    o1 o2
+    (REL: euttOrd_le' o1 (ord_observe o2))
+  : euttOrd_lt' o1 (OStepF o2)
+| euttOrd_tau
+    o1 o2
+    (REL: euttOrd_lt' o1 (ord_observe o2))
+  : euttOrd_lt' o1 (OTauF o2)
+.
+Hint Constructors euttOrd_lt'.
+
+Definition euttOrd_lt o1 o2 := euttOrd_lt' (ord_observe o1) (ord_observe o2).
+Hint Unfold euttOrd_lt.
+
+Lemma euttOrd_lt_le: forall i j, euttOrd_lt i j -> euttOrd_le i j.
+Proof.
+  unfold euttOrd_le, euttOrd_lt. intros i j.
+  generalize (ord_observe i) as oi, (ord_observe j) as oj.
+  intros. induction H; eauto.
+Qed.
+
+Lemma euttOrd_le_le_le: forall i j k, euttOrd_le i j -> euttOrd_le j k -> euttOrd_le i k.
+Proof.
+  unfold euttOrd_le. intros i j k.
+  generalize (ord_observe i) as oi, (ord_observe j) as oj, (ord_observe k) as ok.
+  intros. revert ok H0.
+  induction H; eauto; intros.
+  - remember (OStepF o2) as o2' in *. induction H0; subst; eauto.
+  - remember (OTauF o2) as o2' in *. induction H0; subst; eauto.
+Qed.
+
+Lemma euttOrd_lt_le_lt: forall i j k, euttOrd_lt i j -> euttOrd_le j k -> euttOrd_lt i k.
+Proof.
+  unfold euttOrd_le, euttOrd_lt. intros i j k.
+  generalize (ord_observe i) as oi, (ord_observe j) as oj, (ord_observe k) as ok.
+  intros. revert ok H0.
+  induction H; eauto; intros.
+  - remember (OStepF o2) as o2' in *. induction H0; subst; eauto.
+    econstructor. eapply (euttOrd_lt_le (ord_go _)). eauto.
+  - remember (OTauF o2) as o2' in *. induction H0; subst; eauto.
+    econstructor. eapply (euttOrd_lt_le (ord_go _)). eauto.
+Qed.
+
+Lemma euttOrd_le_lt_lt: forall i j k, euttOrd_le i j -> euttOrd_lt j k -> euttOrd_lt i k.
+Proof.
+  unfold euttOrd_le, euttOrd_lt. intros i j k.
+  generalize (ord_observe i) as oi, (ord_observe j) as oj, (ord_observe k) as ok.
+  intros. revert oi H.
+  induction H0; eauto; intros.
+  econstructor. eapply (euttOrd_le_le_le (ord_go _) (ord_go _)); eauto.
+Qed.
+
+Program Definition euttOrdWf : bwfo :=
+  {| bwfo_set := sig (Acc euttOrd_lt);
+     bwfo_le o1 o2 := euttOrd_le o1 o2;
+     bwfo_lt o1 o2 := euttOrd_lt o1 o2;
+  |}.
+Next Obligation. eauto using euttOrd_lt_le. Qed.
+Next Obligation. eauto using euttOrd_le_le_le. Qed.
+Next Obligation. eauto using euttOrd_lt_le_lt. Qed.
+Next Obligation. eauto using euttOrd_le_lt_lt. Qed.
+Next Obligation.
+  red; intros. destruct a as [o WFo].
+  generalize WFo. induction WFo as [o' _ HYP]. intros.
+  econstructor; intros. destruct y as [y WFy]. eauto.
+Qed.
+
+CoFixpoint eutt_ord {E R1 R2} (ot1: itree' E R1) (ot2: itree' E R2) : euttOrd :=
+  match ot1, ot2 with
+  | TauF t1', TauF t2' => OTau (eutt_ord (observe t1') (observe t2'))
+  | TauF t1', _ => OStep (eutt_ord (observe t1') ot2)
+  | _, TauF t2' => OStep (eutt_ord ot1 (observe t2'))
+  | _, _ => OBase
+  end.
+
+Lemma eutt_ord_wf {E b1 b2 R1 R2 RR o t1 t2}
+      (REL: @eqiti E b1 b2 R1 R2 RR o t1 t2):
+  Acc euttOrd_lt (eutt_ord (observe t1) (observe t2)).
+Proof.
+  revert t1 t2 REL. assert (WF:= wfo_wf gwfo o).
+  induction WF as [o ACC HYP]. intros.
+  econstructor. intros. red in H.
+  remember (ord_observe y) as oy.
+  remember (ord_observe (eutt_ord (observe t1) (observe t2))) as ot.
+  revert t1 t2 REL y Heqoy Heqot. induction H; intros.
+  - punfold REL0. red in REL0. revert_until REL0.
+    inv REL0; intros; subst; try (inv Heqot; fail); pclearbot.
+    + assert (EQo2: o2 = eutt_ord (observe t0) (observe t3)).
+      { destruct (observe t3); inv Heqot; eauto. }
+      subst. econstructor. intros. eapply HYP; eauto using euttOrd_lt_le_lt.
+    + assert (EQo2: o2 = eutt_ord (observe t0) (observe t3)).
+      { destruct (observe t0); inv Heqot; eauto. }
+      subst. econstructor. intros. eapply HYP; eauto using euttOrd_lt_le_lt.
+    + econstructor; intros.
+      eapply (HYP _ LTo _ _ REL1).
+      eapply euttOrd_lt_le_lt; eauto.
+      eapply euttOrd_le_le_le; eauto.
+      red. rewrite <- Heqot. eauto.
+  - subst. genobs t1 ot1. genobs t2 ot2.
+    destruct ot1, ot2; inversion Heqot.
+    eapply IHeuttOrd_lt'; [| |rewrite <- H1]; eauto.
+    eapply eqiti_inv_tauLR.
+    punfold REL. pfold. red. rewrite Heqot1, Heqot2. eauto.
+Qed.
+
+Lemma eqiti_lower_order {E b1 b2 R1 R2 RR o t1 t2}
+      (REL: @eqiti E b1 b2 R1 R2 RR o t1 t2):
+  exists so: euttOrdWf, eqiti b1 b2 RR (gwf_embed so) t1 t2.
+Proof.
+  exists (exist _ (eutt_ord (observe t1) (observe t2)) (eutt_ord_wf REL)).
+  revert_until b2. pcofix CIH. intros.
+  generalize (eutt_ord_wf REL) as WF.  
+  revert_until o. assert (WFo := wfo_wf _ o). induction WFo as [o _ HYP]. intros.
+  revert WF. punfold REL. pfold. red. inv REL; intros.
+  - eauto.
+  - econstructor. intros. specialize (REL0 v). destruct REL0. eauto.
+  - pclearbot. econstructor; eauto.
+    eapply gwf_embed_le_preserve. do 2 econstructor.
+  - genobs t3 ot3. destruct ot3.
+    + unfold_eta. eapply EqTauL; eauto.
+      eapply gwf_embed_lt_preserve. do 2 econstructor.
+    + econstructor. right. eapply CIH.
+      eapply gwf_embed_le_preserve. do 2 econstructor.
+    + unfold_eta. eapply EqTauL; eauto.
+      eapply gwf_embed_lt_preserve. do 2 econstructor.
+  - genobs t0 ot0. destruct ot0.
+    + unfold_eta. eapply EqTauR; eauto.
+      eapply gwf_embed_lt_preserve. do 2 econstructor.
+    + econstructor. right. eapply CIH.
+      eapply gwf_embed_le_preserve. do 2 econstructor.
+    + unfold_eta. eapply EqTauR; eauto.
+      eapply gwf_embed_lt_preserve. do 2 econstructor.
+  - pclearbot. hexploit HYP; eauto. intros EQIT. punfold EQIT.
+Grab Existential Variables.
+  { pclearbot. simpl in *. rewrite Heqot0. punfold REL0. }
+  { pclearbot. punfold REL0. red in REL0. rewrite <-Heqot0 in REL0.
+    destruct b2; inversion CHECK. eauto using eqiti_inv_tauL. }
+  { pclearbot. simpl in *. rewrite Heqot0. punfold REL0. }
+  { pclearbot. simpl in *. rewrite Heqot3. punfold REL0. }
+  { pclearbot. punfold REL0. red in REL0. rewrite <-Heqot3 in REL0.
+    destruct b1; inversion CHECK. eauto using eqiti_inv_tauR. }
+  { pclearbot. simpl in *. rewrite Heqot3. punfold REL0. }
+  { pclearbot. eauto. }
+  { pclearbot. eauto. }
+Qed.
+
+Lemma eqit_lower_order {E b1 b2 R1 R2 RR t1 t2}
+      (REL: @eqit E b1 b2 R1 R2 RR t1 t2):
+  exists so: euttOrdWf, eqiti b1 b2 RR (gwf_embed so) t1 t2.
+Proof. destruct REL. eauto using eqiti_lower_order. Qed.
+
+Lemma euttOrd_small n (so: euttOrdWf) :
+  wfo_lt (gwf_embed so) (wfo_nat (S (S n))).
+Proof.
+  econstructor. simpl. nia.
+Qed.
+
+Lemma eq_itree_zero {E} b1 b2 R1 R2 RR t1 t2
+      (REL: @eq_itree E R1 R2 RR t1 t2):
+  eqiti b1 b2 RR wfo_zero t1 t2.
+Proof.
+  revert_until b2. pcofix CIH. intros.
+  destruct REL. punfold REL. pstep. red.
+  inv REL; try inv CHECK; try inv CHECK1; eauto.
+  - econstructor; eauto.
+    intros. destruct (REL0 v). pclearbot.
+    eexists. left. eapply paco6_mon_bot; [|eauto].
+    eapply eqiti_mon; eauto with wfo_refl; destruct b1, b2; eauto.
+  - econstructor; eauto using wfo_non_negative.
+    pclearbot. right. eauto.
+Qed.
+
+(********************************)
+(** *** Eqit "Up-to" Principles *)
+(********************************)
+
+(* Bind Closure *)
+
+Variant eqit_bind_rel {E} r s R1 R2 (RR:R1->R2->Prop) :
+  gwfo -> itree E R1 -> itree E R2 -> Prop :=
+| eqit_bind_split o o1 o2 U1 U2 (RU : U1 -> U2 -> Prop) t1 t2 k1 k2
+    (EQV: r U1 U2 RU o1 t1 t2 : Prop)
+    (REL: forall u1 u2, RU u1 u2 -> s R1 R2 RR o2 (k1 u1) (k2 u2) : Prop)
+    (LEo: wfo_le (wfo_add o1 o2) o)
+: eqit_bind_rel r s R1 R2 RR o (ITree.bind t1 k1) (ITree.bind t2 k2)
+.
+Hint Constructors eqit_bind_rel: core.
+Arguments eqit_bind_split {E r s R1 R2 RR}.
+
+Definition eqit_bind_clo {E} r := @eqit_bind_rel E r r.
+Hint Unfold eqit_bind_clo: core.
+
+Lemma eqit_bind_rel_monotone {E} r r' s s' R1 R2 RR o o' x y
+      (REL: @eqit_bind_rel E r s R1 R2 RR o x y)
+      (LEr: r <6= r')
+      (LEs: s <6= s')
+      (LEo: wfo_le o o')
+  : eqit_bind_rel r' s' R1 R2 RR o' x y.
+Proof.
+  dependent destruction REL.
+  econstructor; eauto 7 using wfo_le_le_le.
+Qed.
+
+Lemma eqit_bind_clo_prespectful {E} b1 b2:
+  prespectful6 (@eqit_ E b1 b2) eqit_bind_clo.
+Proof.
+  econstructor; repeat intro.
+  - eapply eqit_bind_rel_monotone; eauto using wfo_le_refl.
+  - red in PR. eapply eqit_bind_rel_monotone in PR; [|apply GF|intros; apply PR0|eauto using wfo_le_refl].
+    pstep. red. inversion PR; subst.
+    rewrite !unfold_bind_. inversion EQV.
+    + specialize (REL _ _ REL0). apply GF in REL.
+      eapply eqitF_mono; eauto using rclo6.
+      eapply wfo_le_le_le, LEo; apply wfo_add_proj_right.
+    + econstructor. intros. destruct (REL0 v). eauto 9 using wfo_le_refl.      
+    + simpl. red in EQV.
+      econstructor; [eauto 8 using wfo_le_refl, rclo6|].
+      eapply wfo_le_le_le; [|eauto].
+      eapply wfo_add_le_left; eauto.
+    + rewrite <-unfold_bind_. econstructor; eauto 8 using wfo_le_refl. cycle 1.
+      eapply wfo_lt_le_lt; eauto. eapply wfo_add_lt_left; eauto.
+    + rewrite <-unfold_bind_. econstructor; eauto 8 using wfo_le_refl.
+      eapply wfo_lt_le_lt; eauto. eapply wfo_add_lt_left; eauto.
+    + rewrite <-!unfold_bind_. econstructor; eauto.
+      * right. right. econstructor; eauto using wfo_le_refl.
+      * eauto with wfo.
+Qed.
+
+Lemma eqit_clo_bind E b1 b2:
+  @eqit_bind_clo E <7= gupaco6 (eqit_ b1 b2) (cpn6 (eqit_ b1 b2)).
+Proof.
+  intros. eapply prespect6_uclo; eauto using eqit_bind_clo_prespectful with paco.
+Qed.
+
+Arguments eqit_clo_bind : clear implicits.
+
+(* Transitivity Closure *)
+
+Inductive eqit_transL_clo {E} b b'
+          (r: forall R1 R2,(R1->R2->Prop)-> gwfo -> itree E R1 -> itree E R2 -> Prop)
+          R1 R2 (RR: R1->R2->Prop) o (t1: itree E R1) (t2: itree E R2) : Prop :=
+| eqit_transL_clo_intro o' o1 R1' R1R1' R1'R2 (t1': itree E R1')
+      (EQVl: @eqiti E b b' R1 R1' R1R1' o1 t1 t1')
+      (REL: r R1' R2 R1'R2 o' t1' t2 : Prop)
+      (LEo: wfo_le (wfo_add o' o1) o)
+      (LERR: forall t1 t2 t1', R1R1' t1 t1' -> R1'R2 t1' t2 -> RR t1 t2)
+  : eqit_transL_clo b b' r R1 R2 RR o t1 t2
+.
+Hint Constructors eqit_transL_clo: core.
+
+Inductive eqit_transR_clo {E} b b'
+          (r: forall R1 R2,(R1->R2->Prop)-> gwfo -> itree E R1 -> itree E R2 -> Prop)
+          R1 R2 (RR: R1->R2->Prop) o (t1: itree E R1) (t2: itree E R2) : Prop :=
+| eqit_transR_clo_intro o' o2 R2' R2R2' R1R2' (t2': itree E R2')
+      (EQVr: @eqiti E b b' R2 R2' R2R2' o2 t2 t2')
+      (REL: r R1 R2' R1R2' o' t1 t2' : Prop)
+      (LERR2: forall t1 t2 t2', R2R2' t2 t2' -> R1R2' t1 t2' -> RR t1 t2)
+      (LEo: wfo_le (wfo_add o' o2) o)      
+  : eqit_transR_clo b b' r R1 R2 RR o t1 t2
+.
+Hint Constructors eqit_transR_clo: core.
+
+Lemma eqit_transL_clo_monotone {E} b b' r r' R1 R2 RR o o' x y
+      (REL: @eqit_transL_clo E b b' r R1 R2 RR o x y)
+      (LEr: r <6= r')
+      (LEo: wfo_le o o')
+  : eqit_transL_clo b b' r' R1 R2 RR o' x y.
+Proof.
+  dependent destruction REL.
+  econstructor; eauto 7 using wfo_le_le_le.
+Qed.
+
+Lemma eqit_transR_clo_monotone {E} b b' r r' R1 R2 RR o o' x y
+      (REL: @eqit_transR_clo E b b' r R1 R2 RR o x y)
+      (LEr: r <6= r')
+      (LEo: wfo_le o o')
+  : eqit_transR_clo b b' r' R1 R2 RR o' x y.
+Proof.
+  dependent destruction REL.
+  econstructor; eauto 7 using wfo_le_le_le.
+Qed.
+
+Lemma eqit_transL_clo_prespectful {E} bL bR:
+  prespectful6 (@eqit_ E bL bR) (@eqit_transL_clo E bL bR).
+Proof.
+  econstructor.
+  { repeat intro; eapply eqit_transL_clo_monotone; eauto using wfo_le_refl. }
+
+  intros ? ? ? ? R1 R2 RR o t1 t2 [].
+  eapply paco6_mon; [|intros; right; apply PR].
+  assert (GFl := GF _ _ _ _ _ _ REL).
+  punfold EQVl. pstep. red in GFl, EQVl |- *.
+
+  revert EQVl. inversion GFl; intros; subst.
+
+  (* [Ret] t1' = Ret r1, t2 = Ret r2 *)
+  { inversion EQVl; subst; eauto; pclearbot.
+    (* [TauL] t1 = Tau t0 *)
+    { unfold_eta. eapply EqTauL; eauto; cycle 1.
+      { instantiate (1:= o'0). eauto with wfo wfo_proj. }
+      punfold REL1. red in REL1. rewrite H3 in REL1. left. pstep. red.
+      revert REL1. clear H2. revert t0.
+      assert (WF := wfo_wf _ o'0). induction WF as [ord _ HYP]. intros.
+      dependent destruction REL1.
+      - rewrite <-x. econstructor. eauto.
+      - rewrite <-x0. econstructor; eauto. left. pstep.
+        pclearbot. punfold REL1. red in REL1. rewrite x in REL1.
+        eapply HYP; eauto. eauto with wfo.
+      - econstructor; eauto. left. pstep.
+        pclearbot. punfold REL1. red in REL1. rewrite x, x0 in REL1. 
+        eapply HYP; eauto. eauto with wfo.
+    }
+    (* [Stutter] t1 = t0 *)
+    { unfold_eta. eapply EqStutter; eauto; cycle 1.
+      { instantiate (1:= o'0). eauto with wfo wfo_proj. }
+      punfold REL1. red in REL1. rewrite H3 in REL1. left. pstep. red.
+      revert REL1. clear H2. revert t0.
+      assert (WF := wfo_wf _ o'0). induction WF as [ord _ HYP]. intros.
+      dependent destruction REL1.
+      - rewrite <-x. econstructor. eauto.
+      - rewrite <-x0. econstructor; eauto. left. pstep.
+        pclearbot. punfold REL1. red in REL1. rewrite x in REL1.
+        eapply HYP; eauto. eauto with wfo.
+      - econstructor; eauto. left. pstep.
+        pclearbot. punfold REL1. red in REL1. rewrite x, x0 in REL1. 
+        eapply HYP; eauto. eauto with wfo.
+    }
+  }
+  
+  (* [Vis] t1' = Vis e k1, t2 = Vis e k2 *)
+  { dependent destruction EQVl; pclearbot. 
+    (* [Vis] t1 = Vis e k0 *)
+    { rewrite <-x. eapply EqVis; intros.
+      destruct (REL0 v), (REL1 v); pclearbot.
+      eexists. right. econstructor; eauto with wfo_refl.
+    }
+    (* [TauL] t1 = Tau t0 *)
+    { rewrite <-x0. unfold_eta. econstructor; eauto; cycle 1.
+      { instantiate (1:= o'0). eauto with wfo wfo_proj. }
+      punfold REL1. red in REL1. rewrite x in REL1. left. pstep. red.
+      revert REL1. clear x0. revert t0.
+      assert (WF := wfo_wf _ o'0). induction WF as [ord _ HYP]. intros.
+      dependent destruction REL1.
+      - rewrite <-x. econstructor. intros.
+        destruct (REL0 v). destruct (REL1 v). pclearbot. 
+        eexists (wfo_add _ _).
+        right. econstructor; eauto with wfo_refl.
+      - rewrite <-x1. econstructor; eauto. left. pstep.
+        pclearbot. punfold REL1. red in REL1. rewrite x in REL1.
+        eapply HYP; eauto. eauto with wfo.
+      - econstructor; eauto. left. pstep.
+        pclearbot. punfold REL1. red in REL1. rewrite x, x1 in REL1.
+        eapply HYP; eauto. eauto with wfo.
+    }
+    (* [Stutter] t1 = t0 *)
+    { rewrite <-x0. unfold_eta. econstructor; eauto; cycle 1.
+      { instantiate (1:= o'0). eauto with wfo wfo_proj. }
+      punfold REL1. red in REL1. rewrite x in REL1. left. pstep. red.
+      revert REL1. clear x0. revert t0.
+      assert (WF := wfo_wf _ o'0). induction WF as [ord _ HYP]. intros.
+      dependent destruction REL1.
+      - rewrite <-x. econstructor. intros.
+        destruct (REL0 v). destruct (REL1 v). pclearbot. 
+        eexists (wfo_add _ _).
+        right. econstructor; eauto with wfo_refl.
+      - rewrite <-x1. econstructor; eauto. left. pstep.
+        pclearbot. punfold REL1. red in REL1. rewrite x in REL1.
+        eapply HYP; eauto. eauto with wfo.
+      - econstructor; eauto. left. pstep.
+        pclearbot. punfold REL1. red in REL1. rewrite x, x1 in REL1.
+        eapply HYP; eauto. eauto with wfo.
+    }
+  }
+  
+  (* [Tau] t1' = Tau m1, t2 = Tau m2 *)
+  { inversion EQVl; subst; eauto; pclearbot.
+    (* [Tau] t1 = Tau m0 *)
+    { econstructor; eauto 7 with wfo.
+    }
+    (* [TauL] t1 = Tau t0 *)
+    { destruct bL; inv CHECK.
+      hexploit eqiti_inv_tauR.
+      { pstep. rewrite <-H3. punfold REL1. }
+      { eauto. }
+      intros RELt0m1.
+      econstructor.
+      - right. econstructor; eauto with wfo_refl.
+      - eauto with wfo.
+    }
+    (* [TauR] t1 = Tau t0 *)
+    { econstructor; eauto.
+      - right. econstructor; eauto using wfo_le_refl.
+      - eauto 8 with wfo.
+    }
+    (* [Stutter] t1 = Tau t0 *)
+    { destruct bL, bR; inv CHECK1; inv CHECK2.
+      unfold_eta. eapply EqStutter; eauto with wfo.
+      punfold REL1. red in REL1. rewrite H3 in REL1. left. pstep. red.
+      remember (wfo_add o'1 o'0) as ord. clear H2. revert o'1 t0 LTo REL1 Heqord.
+      assert (WF := wfo_wf _ ord). induction WF as [ord _ HYP]. intros.
+      dependent destruction REL1; pclearbot.
+      - rewrite <-x. econstructor.
+        + right. econstructor; eauto with wfo_refl.
+        + subst. eauto with wfo.
+      - rewrite <-x0. econstructor.
+        right. econstructor; try apply REL0; eauto with wfo_refl.
+        + eapply eqiti_inv_tauR; eauto.
+          pstep. red. rewrite <-x. punfold REL1.
+        + subst. eauto with wfo_refl.
+      - rewrite <-x. econstructor; eauto.
+        + right. econstructor; eauto with wfo_refl.
+        + subst. eauto with wfo.
+      - rewrite <-x0. eapply EqStutter; eauto.
+        + left. pstep. punfold REL1. red in REL1. rewrite x in REL1.
+          eapply HYP; try apply REL1; subst; eauto; eauto with wfo.
+        + subst. eauto with wfo.
+    }
+  }
+  
+  (* [TauL] t1' = Tau t0, t2 = t3 *)
+  { inversion EQVl; subst; eauto; pclearbot.
+    (* [Tau] t1 = Tau m1 *)
+    { econstructor; eauto.
+      + right. econstructor; eauto with wfo_refl.
+      + eauto with wfo.
+    }
+    (* [TauL] t1 = Tau t4 *)
+    { destruct bL; inv CHECK.
+      hexploit eqiti_inv_tauR.
+      { pstep. rewrite <-H3. punfold REL1. }
+      { eauto. }
+      intros RELt0m1.
+      econstructor; eauto.
+      - right. econstructor; eauto with wfo_refl.
+      - eauto with wfo.
+    }
+    (* [TauR] t1 = t4 *)
+    { econstructor; eauto.
+      - right. econstructor; eauto using wfo_le_refl.
+      - eauto 8 with wfo.
+    }
+    (* [Stutter] t1 = t4 *)
+    { destruct bL, bR; inv CHECK1; inv CHECK2.
+      eapply EqStutter; eauto.
+      - right. econstructor; cycle 1; eauto with wfo_refl.
+        eapply eqiti_inv_tauR; eauto.
+        rewrite <-H3. pstep. punfold REL1.
+      - eauto with wfo.
+    }
+  }
+
+  (* [TauR] t1' = t0, t2 = Tau t3 *)
+  { econstructor; eauto 7 with wfo wfo_refl.
+  }
+  
+  (* [Stutter] ... *)
+  { econstructor; eauto 7 with wfo wfo_refl.
+  }
+Qed.
+
+Lemma eqit_transR_clo_prespectful {E} bL bR:
+  prespectful6 (@eqit_ E bL bR) (@eqit_transR_clo E bR bL).
+Proof.
+  econstructor.
+  { repeat intro; eapply eqit_transR_clo_monotone; eauto using wfo_le_refl. }
+
+  intros ? ? ? ? R1 R2 RR o t1 t2 CLO.
+  apply eqiti_r_flip.
+  eapply paco6_mon.
+  - eapply eqit_transL_clo_prespectful.
+    + instantiate (1:= eqit_rel_flip r).
+      instantiate (1:= eqit_rel_flip l).
+      unfold eqit_rel_flip. eauto.
+    + unfold eqit_rel_flip. intros.
+      apply GF in PR. eauto using eqitF_flip.
+    + destruct CLO. econstructor; eauto.
+      * instantiate (1:= flip R1R2'). eauto.
+      * eauto.
+  - unfold eqit_rel_flip.
+    intros. destruct PR; eauto.
+    right. destruct H. econstructor; eauto.
+Qed.
+
+Lemma eqit_clo_transL E bL bR:
+  @eqit_transL_clo E bL bR <7= gupaco6 (eqit_ bL bR) (cpn6 (eqit_ bL bR)).
+Proof.
+  intros. eapply prespect6_uclo; eauto using eqit_transL_clo_prespectful with paco.
+Qed.
+
+Lemma eqit_clo_transR E bL bR:
+  @eqit_transR_clo E bR bL <7= gupaco6 (eqit_ bL bR) (cpn6 (eqit_ bL bR)).
+Proof.
+  intros. eapply prespect6_uclo; eauto using eqit_transR_clo_prespectful with paco.
+Qed.
+
+Arguments eqit_clo_transL : clear implicits.
+Arguments eqit_clo_transR : clear implicits.
+
+(** *** Bind properties *)
+
+Lemma eutt_clo_bind {E U1 U2 UU R1 R2 RR} t1 t2 k1 k2
+      (EQT: @eutt E U1 U2 UU t1 t2)
+      (EQK: forall u1 u2, UU u1 u2 -> @eutt E R1 R2 RR (k1 u1) (k2 u2)):
+  eutt RR (x <- t1;; k1 x) (x <- t2;; k2 x).
+Proof.
+  intros. destruct (eqit_lower_order EQT) as [so EQTso].
+  eexists. ginit. guclo eqit_clo_bind.
+  econstructor; eauto using wfo_le_refl with paco.
+  intros. destruct (eqit_lower_order (EQK _ _ H)) as [so' RELso'].
+  gfinal. right.
+  eapply eqiti_mon; eauto using wfo_lt_le, (euttOrd_small 0).
 Qed.
 
 (** *** Transitivity properties *)
 
-Inductive rcompose {R1 R2 R3} (RR1: R1->R2->Prop) (RR2: R2->R3->Prop) (r1: R1) (r3: R3) : Prop :=
-| rcompose_intro r2 (REL1: RR1 r1 r2) (REL2: RR2 r2 r3)
-.
-Hint Constructors rcompose: core.
-
-Lemma trans_rcompose {R} RR (TRANS: Transitive RR):
-  forall x y : R, rcompose RR RR x y -> RR x y.
+Lemma eqiti_trans {E} b1 b2 {R1 R2 R3} (RR1: R1->R2->Prop) (RR2: R2->R3->Prop) (RR: R1->R3->Prop) o1 o2 o t1 t2 t3
+      (INL: eqiti b1 b2 RR1 o1 t1 t2)
+      (INR: eqiti b1 b2 RR2 o2 t2 t3)
+      (LEo: wfo_le (wfo_add o1 o2) o)
+      (RRComp: forall x y z, RR1 x y -> RR2 y z -> RR x z)
+  : @eqiti E b1 b2 _ _ RR o t1 t3.
 Proof.
-  intros. destruct H; eauto.
+  ginit.
+  guclo eqit_clo_transR. econstructor.
+  - eapply eqiti_flip. instantiate (3:= flip RR2). eauto.
+  - gfinal. eauto.
+  - eauto.
+  - eauto.
 Qed.
 
-Lemma eqit_trans {E R1 R2 R3} (RR1: R1->R2->Prop) (RR2: R2->R3->Prop) b1 b2 t1 t2 t3
-      (INL: eqit RR1 b1 b2 t1 t2)
-      (INR: eqit RR2 b1 b2 t2 t3):
-  @eqit E _ _ (rcompose RR1 RR2) b1 b2 t1 t3.
+Lemma eqit_trans {E} b1 b2 {R1 R2 R3} (RR1: R1->R2->Prop) (RR2: R2->R3->Prop) (RR: R1->R3->Prop) t1 t2 t3
+      (INL: eqit b1 b2 RR1 t1 t2)
+      (INR: eqit b1 b2 RR2 t2 t3)
+      (RRComp: forall x y z, RR1 x y -> RR2 y z -> RR x z)
+  : @eqit E b1 b2 _ _ RR t1 t3.
 Proof.
-  revert_until b2. pcofix CIH. intros.
-  pstep. punfold INL. punfold INR. red in INL, INR |- *. genobs_clear t3 ot3.
-  hinduction INL before CIH; intros; subst; clear t1 t2; eauto.
-  - remember (RetF r2) as ot.
-    hinduction INR before CIH; intros; inv Heqot; eauto with paco.
-  - assert (DEC: (exists m3, ot3 = TauF m3) \/ (forall m3, ot3 <> TauF m3)).
-    { destruct ot3; eauto; right; red; intros; inv H. }
-    destruct DEC as [EQ | EQ].
-    + destruct EQ as [m3 ?]; subst.
-      econstructor. right. pclearbot. eapply CIH; eauto with paco.
-      eapply eqit_inv_tauLR. eauto.
-    + inv INR; try (exfalso; eapply EQ; eauto; fail).
-      econstructor; eauto.
-      pclearbot. punfold REL. red in REL.
-      hinduction REL0 before CIH; intros; try (exfalso; eapply EQ; eauto; fail).
-      * remember (RetF r1) as ot.
-        hinduction REL0 before CIH; intros; inv Heqot; eauto with paco.
-      * remember (VisF e k1) as ot.
-        hinduction REL0 before CIH; intros; dependent destruction Heqot; eauto with paco.
-        econstructor. intros. right.
-        destruct (REL v), (REL0 v); try contradiction. eauto.
-      * eapply IHREL0; eauto. pstep_reverse.
-        destruct b1; inv CHECK0.
-        apply eqit_inv_tauR. eauto.
-  - remember (VisF e k2) as ot.
-    hinduction INR before CIH; intros; dependent destruction Heqot; eauto.
-    econstructor. intros.
-    destruct (REL v), (REL0 v); try contradiction; eauto.
-  - remember (TauF t0) as ot.
-    hinduction INR before CIH; intros; dependent destruction Heqot; eauto.
-    eapply IHINL; eauto. pclearbot. punfold REL.
+  destruct INL, INR. eexists.
+  eapply eqiti_trans; eauto with wfo_refl.
+Qed.
+
+Lemma eutt_trans {E} {R1 R2 R3} (RR1: R1->R2->Prop) (RR2: R2->R3->Prop) (RR: R1->R3->Prop) t1 t2 t3
+      (INL: eutt RR1 t1 t2)
+      (INR: eutt RR2 t2 t3)
+      (RRComp: forall x y z, RR1 x y -> RR2 y z -> RR x z)
+  : @eutt E _ _ RR t1 t3.
+Proof.
+  destruct INL, INR. eexists.
+  eapply eqiti_trans; eauto with wfo_refl.
 Qed.
 
 Global Instance Transitive_eqit {E : Type -> Type} {R: Type} (RR : R -> R -> Prop) (b1 b2: bool):
-  Transitive RR -> Transitive (@eqit E _ _ RR b1 b2).
+  Transitive RR -> Transitive (@eqit E b1 b2 _ _ RR).
 Proof.
-  red; intros. eapply eqit_mon, eqit_trans; eauto using (trans_rcompose RR).
+  red; intros. eapply eqit_mon; [eapply eqit_trans|..]; eauto.
 Qed.
 
 Global Instance Transitive_eqit_eq {E : Type -> Type} {R: Type} (b1 b2: bool):
-  Transitive (@eqit E R R eq b1 b2).
+  Transitive (@eqit E b1 b2 R R eq).
 Proof.
   apply Transitive_eqit. repeat intro; subst; eauto.
 Qed.
 
 Global Instance Equivalence_eqit {E : Type -> Type} {R: Type} (RR : R -> R -> Prop) (b: bool):
-  Equivalence RR -> Equivalence (@eqit E R R RR b b).
+  Equivalence RR -> Equivalence (@eqit E b b R R RR).
 Proof.
   constructor; try typeclasses eauto.
 Qed.
 
 Global Instance Equivalence_eqit_eq {E : Type -> Type} {R: Type} (b: bool):
-  Equivalence (@eqit E R R eq false false).
+  Equivalence (@eqit E false false R R eq).
 Proof.
   constructor; try typeclasses eauto.
 Qed.
 
 Global Instance Transitive_eutt {E R RR} : Transitive RR -> Transitive (@eutt E R R RR).
 Proof.
-  red; intros. eapply eqit_mon, eqit_trans; eauto using (trans_rcompose RR).
+  red; intros. eapply eqit_mon; [eapply eqit_trans|..]; eauto.
 Qed.
 
 Global Instance Equivalence_eutt {E R RR} : Equivalence RR -> Equivalence (@eutt E R R RR).
@@ -815,24 +1461,25 @@ Proof.
   constructor; try typeclasses eauto.
 Qed.
 
-Global Instance geuttgen_cong_eqit {E R1 R2 RR1 RR2 RS} b1 b2 r rg
+Global Instance geuttgen_cong_eqit {E R1 R2 RR1 RR2 RS} b1 b2 r rg o
        (LERR1: forall x x' y, (RR1 x x': Prop) -> (RS x' y: Prop) -> RS x y)
        (LERR2: forall x y y', (RR2 y y': Prop) -> RS x y' -> RS x y):
   Proper (eq_itree RR1 ==> eq_itree RR2 ==> flip impl)
-         (gpaco2 (@eqit_ E R1 R2 RS b1 b2 id) (eqitC RS b1 b2) r rg).
+         (gpaco6 (@eqit_ E b1 b2) (cpn6 (eqit_ b1 b2)) r rg R1 R2 RS o).
 Proof.
-  repeat intro. guclo eqit_clo_trans. econstructor; cycle -3; eauto.
-  - eapply eqit_mon, H; eauto; discriminate.
-  - eapply eqit_mon, H0; eauto; discriminate.
+  repeat intro.
+  guclo eqit_clo_transL. econstructor; eauto using eq_itree_zero, wfo_add_zero_r_le.
+  guclo eqit_clo_transR. econstructor; eauto using eq_itree_zero, wfo_add_zero_r_le.
 Qed.
 
-Global Instance geuttgen_cong_eqit_eq {E R1 R2 RS} b1 b2 r rg:
+Global Instance geuttgen_cong_eqit_eq {E R1 R2 RS} b1 b2 r rg o:
   Proper (eq_itree eq ==> eq_itree eq ==> flip impl)
-         (gpaco2 (@eqit_ E R1 R2 RS b1 b2 id) (eqitC RS b1 b2) r rg).
+         (gpaco6 (@eqit_ E b1 b2) (cpn6 (eqit_ b1 b2)) r rg R1 R2 RS o).
 Proof.
   eapply geuttgen_cong_eqit; intros; subst; eauto.
 Qed.
 
+(*
 Global Instance geuttge_cong_euttge {E R1 R2 RR1 RR2 RS} r rg
        (LERR1: forall x x' y, (RR1 x x': Prop) -> (RS x' y: Prop) -> RS x y)
        (LERR2: forall x y y', (RR2 y y': Prop) -> RS x y' -> RS x y):
@@ -860,38 +1507,41 @@ Qed.
 
 Global Instance geutt_cong_euttge_eq {E R1 R2 RS} r rg:
   Proper (euttge eq ==> euttge eq ==> flip impl)
-         (gpaco2 (@eqit_ E R1 R2 RS true true id) (eqitC RS true true) r rg).
+         (gpaco2 (@eqit_ E true true R1 R2 RS id) (eqitC RS true true) r rg).
 Proof.
   eapply geutt_cong_euttge; intros; subst; eauto.
 Qed.
+*)
 
 Global Instance eqitgen_cong_eqit {E R1 R2 RR1 RR2 RS} b1 b2
        (LERR1: forall x x' y, (RR1 x x': Prop) -> (RS x' y: Prop) -> RS x y)
        (LERR2: forall x y y', (RR2 y y': Prop) -> RS x y' -> RS x y):
   Proper (eq_itree RR1 ==> eq_itree RR2 ==> flip impl)
-         (@eqit E R1 R2 RS b1 b2).
+         (@eqit E b1 b2 R1 R2 RS).
 Proof.
-  ginit. intros. eapply geuttgen_cong_eqit; eauto. gfinal. eauto.
+  repeat intro. destruct H1. eexists.
+  ginit. eapply geuttgen_cong_eqit; eauto. gfinal. eauto.
 Qed.
 
 Global Instance eqitgen_cong_eqit_eq {E R1 R2 RS} b1 b2:
   Proper (eq_itree eq ==> eq_itree eq ==> flip impl)
          (@eqit E R1 R2 RS b1 b2).
 Proof.
-  ginit. intros. rewrite H1, H0. gfinal. eauto.
+  repeat intro. destruct H1. eexists.
+  ginit. intros. rewrite H, H0. gfinal. eauto.
 Qed.
 
 Global Instance euttge_cong_euttge {E R RS}
        (TRANS: Transitive RS):
   Proper (euttge RS ==> flip (euttge RS) ==> flip impl)
-         (@eqit E R R RS true false).
+         (@eqit E true false R R RS).
 Proof.
-  repeat intro. do 2 (eapply eqit_mon, eqit_trans; eauto using (trans_rcompose RS)).
+  repeat intro. do 2 (eapply eqit_mon; [eapply eqit_trans|..]; eauto).
 Qed.
 
 Global Instance euttge_cong_euttge_eq {E R}:
   Proper (euttge eq ==> flip (euttge eq) ==> flip impl)
-         (@eqit E R R eq true false).
+         (@eqit E true false R R eq).
 Proof.
   eapply euttge_cong_euttge; eauto using eq_trans.
 Qed.
@@ -922,10 +1572,11 @@ Lemma bind_trigger {E R} U (e : E U) (k : U -> itree E R)
   : ITree.bind (ITree.trigger e) k ≅ Vis e (fun x => k x).
 Proof.
   rewrite unfold_bind; cbn.
-  pstep.
+  eexists. ginit. gstep.
   constructor.
-  intros; red. left. rewrite bind_ret_l.
-  apply Reflexive_eqit; eauto.
+  intros; eexists. rewrite bind_ret_l.
+  gfinal. right. eapply Reflexive_eqiti; eauto.
+Grab Existential Variables. exact wfo_zero. exact wfo_zero.
 Qed.
 
 Lemma unfold_iter {E A B} (f : A -> itree E (A + B)) (x : A) :
@@ -941,119 +1592,47 @@ Proof.
   reflexivity.
 Qed.
 
-Ltac auto_ctrans :=
-  intros; repeat (match goal with [H: rcompose _ _ _ _ |- _] => destruct H end); subst; eauto.
-Ltac auto_ctrans_eq := try instantiate (1:=eq); auto_ctrans.
-
-Section eqit_h.
-
-Context {E : Type -> Type} {R1 R2 : Type} (RR : R1 -> R2 -> Prop).
+(* Ltac auto_ctrans := *)
+(*   intros; repeat (match goal with [H: rcompose _ _ _ _ |- _] => destruct H end); subst; eauto. *)
+(* Ltac auto_ctrans_eq := try instantiate (1:=eq); auto_ctrans. *)
 
 (** [eqit] is a congruence for [itree] constructors. *)
-
-Lemma eqit_Tau b1 b2 (t1 : itree E R1) (t2 : itree E R2) :
-  eqit RR b1 b2 (Tau t1) (Tau t2) <-> eqit RR b1 b2 t1 t2.
-Proof.
-  split; intros H.
-  - punfold H. red in H. simpl in *. pstep. red.
-    remember (TauF t1) as ot1. remember (TauF t2) as ot2.
-    hinduction H before RR; intros; subst; try inv Heqot1; try inv Heqot2; eauto.
-    + pclearbot. punfold REL.
-    + inv H; eauto.
-    + inv H; eauto.
-  - pstep. constructor; auto.
-Qed.
-
-Lemma eqit_Vis b1 b2 {U} (e : E U)
-      (k1 : U -> itree E R1) (k2 : U -> itree E R2) :
-      (forall u, eqit RR b1 b2 (k1 u) (k2 u))
-  <-> eqit RR b1 b2 (Vis e k1) (Vis e k2).
-Proof.
-  split; intros H.
-  - pstep. econstructor. left. apply H.
-  - punfold H. inv H; auto_inj_pair2; subst; auto.
-    intros. pclearbot. eauto.
-Qed.
-
-Lemma eqit_Ret b1 b2 (r1 : R1) (r2 : R2) :
-  RR r1 r2 <-> @eqit E _ _ RR b1 b2 (Ret r1) (Ret r2).
-Proof.
-  split; intros H.
-  - pstep. constructor; auto.
-  - punfold H. inversion H; auto_inj_pair2; subst; auto.
-Qed.
-
-(** *** "Up-to" principles for coinduction. *)
-
-Inductive eqit_bind_clo b1 b2 (r : itree E R1 -> itree E R2 -> Prop) :
-  itree E R1 -> itree E R2 -> Prop :=
-| pbc_intro_h U1 U2 (RU : U1 -> U2 -> Prop) t1 t2 k1 k2
-      (EQV: eqit RU b1 b2 t1 t2)
-      (REL: forall u1 u2, RU u1 u2 -> r (k1 u1) (k2 u2))
-  : eqit_bind_clo b1 b2 r (ITree.bind t1 k1) (ITree.bind t2 k2)
-.
-Hint Constructors eqit_bind_clo: core.
-
-Lemma eqit_clo_bind b1 b2 vclo
-      (MON: monotone2 vclo)
-      (CMP: compose (eqitC RR b1 b2) vclo <3= compose vclo (eqitC RR b1 b2))
-      (ID: id <3= vclo):
-  eqit_bind_clo b1 b2 <3= gupaco2 (eqit_ RR b1 b2 vclo) (eqitC RR b1 b2).
-Proof.
-  gcofix CIH. intros. destruct PR.
-  guclo eqit_clo_trans.
-  econstructor; auto_ctrans_eq; try (rewrite (itree_eta (x <- _;; _ x)), unfold_bind; reflexivity).
-  punfold EQV. unfold_eqit.
-  hinduction EQV before CIH; intros; pclearbot.
-  - guclo eqit_clo_trans.
-    econstructor; auto_ctrans_eq; try (rewrite <- !itree_eta; reflexivity).
-    eauto with paco.
-  - gstep. econstructor. eauto with paco.
-  - gstep. econstructor. eauto 7 with paco.
-  - destruct b1; try discriminate.
-    guclo eqit_clo_trans.
-    econstructor; auto_ctrans_eq; cycle -1; eauto; try reflexivity.
-    eapply eqit_tauL. rewrite unfold_bind, <-itree_eta. reflexivity.
-  - destruct b2; try discriminate.
-    guclo eqit_clo_trans. econstructor; auto_ctrans_eq; cycle -1; eauto; try reflexivity.
-    eapply eqit_tauL. rewrite unfold_bind, <-itree_eta. reflexivity.
-Qed.
-
-Lemma eutt_clo_bind {U1 U2 UU} t1 t2 k1 k2
-      (EQT: @eutt E U1 U2 UU t1 t2)
-      (EQK: forall u1 u2, UU u1 u2 -> eutt RR (k1 u1) (k2 u2)):
-  eutt RR (x <- t1;; k1 x) (x <- t2;; k2 x).
-Proof.
-  intros. ginit. guclo eqit_clo_bind.
-  econstructor; eauto. intros; subst. gfinal. right. apply EQK. eauto.
-Qed.
-
-End eqit_h.
 
 Lemma eutt_Tau {E R} (t1 t2 : itree E R):
   Tau t1 ≈ Tau t2 <-> t1 ≈ t2.
 Proof.
-  apply eqit_Tau.
+  apply eqit_tau.
 Qed.
 
 Lemma eqitree_Tau {E R} (t1 t2 : itree E R):
   Tau t1 ≅ Tau t2 <-> t1 ≅ t2.
 Proof.
-  apply eqit_Tau.
+  apply eqit_tau.
 Qed.
 
-Arguments eqit_clo_bind : clear implicits.
-Hint Constructors eqit_bind_clo: core.
+(* Specialization of [eutt_clo_bind] to the recurrent case where [UU := eq]
+   in order to avoid having to provide the relation manually everytime *)
+Lemma eutt_eq_bind : forall E R U (t: itree E U) (k1 k2: U -> itree E R), (forall u, k1 u ≈ k2 u) -> ITree.bind t k1 ≈ ITree.bind t k2.
+Proof.
+  intros. eapply eutt_clo_bind; [reflexivity|].
+  intros; subst. eauto.
+Qed.
 
 Lemma eqit_bind' {E R1 R2 S1 S2} (RR : R1 -> R2 -> Prop) b1 b2
       (RS : S1 -> S2 -> Prop)
       t1 t2 k1 k2 :
-  eqit RR b1 b2 t1 t2 ->
-  (forall r1 r2, RR r1 r2 -> eqit RS b1 b2 (k1 r1) (k2 r2)) ->
-  @eqit E _ _ RS b1 b2 (ITree.bind t1 k1) (ITree.bind t2 k2).
+  eqit b1 b2 RR t1 t2 ->
+  (forall r1 r2, RR r1 r2 -> eqit b1 b2 RS (k1 r1) (k2 r2)) ->
+  @eqit E b1 b2 _ _ RS (ITree.bind t1 k1) (ITree.bind t2 k2).
 Proof.
-  intros. ginit. guclo eqit_clo_bind. unfold eqit in *.
-  econstructor; eauto with paco.
+  intros. eexists.
+  ginit. guclo eqit_clo_bind.
+  eapply eqit_bind_split; intros; eauto with wfo_refl.
+  - gfinal. right. destruct (eqit_lower_order H).
+    eapply eqiti_mon; eauto using wfo_lt_le, euttOrd_small.
+  - gfinal. right. destruct (eqit_lower_order (H0 _ _ H1)).
+    eapply eqiti_mon; eauto using wfo_lt_le, euttOrd_small.
+Grab Existential Variables. exact 0. exact 0.
 Qed.
 
 Lemma eq_itree_clo_bind {E : Type -> Type} {R1 R2 : Type} (RR : R1 -> R2 -> Prop) {U1 U2 UU} t1 t2 k1 k2
@@ -1065,40 +1644,43 @@ Proof.
 Qed.
 
 Global Instance eqit_bind {E R S} b1 b2 :
-  Proper (pointwise_relation _ (eqit eq b1 b2) ==>
-          eqit eq b1 b2 ==>
-          eqit eq b1 b2) (@ITree.bind' E R S).
+  Proper (pointwise_relation _ (eqit b1 b2 eq) ==>
+          eqit b1 b2 eq ==>
+          eqit b1 b2 eq) (@ITree.bind' E R S).
 Proof.
   repeat intro; eapply eqit_bind'; eauto.
   intros; subst; auto.
 Qed.
 
 Global Instance eqit_bind_ {E R S} b1 b2 k :
-  Proper (going (eqit eq b1 b2) ==>
-          eqit eq b1 b2) (@ITree._bind E R S k (@ITree.bind' E R S k)).
+  Proper (going (eqit b1 b2 eq) ==>
+          eqit b1 b2 eq) (@ITree._bind E R S k (@ITree.bind' E R S k)).
 Proof.
-  ginit. intros. destruct H0.
+  eexists. ginit. destruct H.
   rewrite (itree_eta' x), (itree_eta' y), <- !unfold_bind.
-  guclo eqit_clo_bind. econstructor; eauto.
-  intros. subst. apply reflexivity.
+  guclo eqit_clo_bind. econstructor; eauto with wfo_refl; intros.
+  - gfinal. right. destruct (eqit_lower_order e).
+    eapply eqiti_mon; eauto using wfo_lt_le, euttOrd_small.
+  - subst. apply reflexivity.
+Grab Existential Variables. exact 0. exact wfo_zero.
 Qed.
 
 Lemma eqit_map {E R1 R2 S1 S2} (RR : R1 -> R2 -> Prop) b1 b2
       (RS : S1 -> S2 -> Prop)
       f1 f2 t1 t2 :
   (forall r1 r2, RR r1 r2 -> RS (f1 r1) (f2 r2)) ->
-  @eqit E _ _ RR b1 b2 t1 t2 ->
-  eqit RS b1 b2 (ITree.map f1 t1) (ITree.map f2 t2).
+  @eqit E b1 b2 _ _ RR t1 t2 ->
+  eqit b1 b2 RS (ITree.map f1 t1) (ITree.map f2 t2).
 Proof.
   unfold ITree.map; intros.
   eapply eqit_bind'; eauto.
-  intros; pstep; constructor; auto.
+  intros. eexists wfo_zero. pstep. econstructor. eauto.
 Qed.
 
 Global Instance eqit_eq_map {E R S} b1 b2 :
   Proper (pointwise_relation _ eq ==>
-          eqit eq b1 b2 ==>
-          eqit eq b1 b2) (@ITree.map E R S).
+          eqit b1 b2 eq ==>
+          eqit b1 b2 eq) (@ITree.map E R S).
 Proof.
   repeat intro; eapply eqit_map; eauto.
   intros; subst; auto.
@@ -1108,9 +1690,10 @@ Lemma bind_ret_r {E R} :
   forall s : itree E R,
     ITree.bind s (fun x => Ret x) ≅ s.
 Proof.
+  eexists wfo_zero. revert R s.
   ginit. gcofix CIH. intros.
   rewrite !unfold_bind. gstep. repeat red.
-  genobs s os. destruct os; simpl; eauto with paco.
+  genobs s os. destruct os; simpl; eauto using wfo_non_negative with paco.
 Qed.
 
 Lemma bind_ret_r' {E R} (u : itree E R) (f : R -> R) :
@@ -1118,9 +1701,11 @@ Lemma bind_ret_r' {E R} (u : itree E R) (f : R -> R) :
   (r <- u ;; Ret (f r)) ≅ u.
 Proof.
   intro H. rewrite <- (bind_ret_r u) at 2. apply eqit_bind.
-  - hnf. intros. apply eqit_Ret. auto.
+  - hnf. intros. apply eqit_ret. auto.
   - reflexivity.
 Qed.
+
+(* ----------------- Revised Up Here ------------------ *)
 
 Lemma bind_bind {E R S T} :
   forall (s : itree E R) (k : R -> itree E S) (h : S -> itree E T),
@@ -1230,7 +1815,7 @@ Proof.
     destruct (observe ma) eqn: Hobma.
     * exists r0. split. rewrite <- Hobma. tau_steps. reflexivity.
       cbn in *. rewrite <- H0. rewrite itree_eta, Hobtl.
-      apply eqit_Ret; auto.
+      apply eqit_ret; auto.
     * cbn in H0. rewrite itree_eta in H0. rewrite Hobtl in H0.
       apply eqitree_inv_ret_tau in H0. contradiction.
     * cbn in H0. rewrite itree_eta, Hobtl in H0.
@@ -1300,7 +1885,7 @@ Proof.
   - intros. rewrite unfold_bind in H0.
     destruct (observe ma) eqn: Hobma; cbn in *; rewrite itree_eta in H0; rewrite <- Heqtl' in H0.
     + right. exists r. split. rewrite itree_eta. rewrite Hobma. reflexivity.
-      rewrite <- H0. apply eqit_Vis.
+      rewrite <- H0. apply eqit_vis.
       intros. destruct (REL u0); auto. inv H.
     + symmetry in H0. apply eqitree_inv_tau_vis in H0. contradiction.
     + setoid_rewrite itree_eta at 1. rewrite Hobma. clear Hobma Heqtl'.
@@ -1389,7 +1974,7 @@ Proof.
     destruct (observe ma) eqn:Hobma.
     + cbn in *.
       right. exists r. rewrite itree_eta. rewrite Hobma. split; [reflexivity |].
-      rewrite <- H0. apply eqit_Tau. pclearbot. auto.
+      rewrite <- H0. apply eqit_tau. pclearbot. auto.
     + cbn in *.
       left. exists t. rewrite itree_eta. rewrite Hobma. split; [reflexivity |].
       rewrite eqitree_Tau in H0. rewrite <- H0. pclearbot. auto.
@@ -1412,7 +1997,7 @@ Proof.
       * left. destruct H1 as (a & ? & ?).
         exists (Ret a). rewrite itree_eta. rewrite Hobma. rewrite H1.
         split; [reflexivity |]. rewrite unfold_bind. cbn.
-        apply eqit_tauL in H2. rewrite <- eqit_Tau. auto.
+        apply eqit_tauL in H2. rewrite <- eqit_tau. auto.
     + cbn in *. apply eqitree_inv_tau_vis in H0; contradiction.
   - intros. subst. inv Heqtr'.
     rewrite unfold_bind in H0.
