theories/Basics/GeneralWFO.v
@@ -1,0 +1,644 @@
+(** Well-founded orders. *)
+
+Require Import Arith Relations Max NPeano Program Wellfounded List Lia.
+From Paco Require Import paco.
+Import ListNotations.
+
+Set Implicit Arguments. 
+Global Set Bullet Behavior "Strict Subproofs".
+
+Ltac ginduction H :=
+  move H at top; revert_until H; induction H.
+
+(** * Additions to the Relations library. *)
+
+Notation rtc := (clos_refl_trans _). (* reflexive transitive closure *)
+Notation tc := (clos_trans _). (* transitive closure *)
+Hint Immediate rt_step rt_refl t_step.
+
+Lemma tc_well_founded: forall A R
+    (WF: @well_founded A R),
+  well_founded (tc R).
+Proof. clear.
+  red; intros; induction a using (well_founded_ind WF); econstructor; intros.
+  apply clos_trans_tn1_iff in H0; induction H0; eauto.
+  apply IHclos_trans_n1; specialize (H y0 H0); inversion H; eauto.
+Qed.
+
+Lemma rtc_mon: forall X (R R': X -> X -> Prop) a b
+    (IN: rtc R a b)
+    (LE: R <2= R'),
+  rtc R' a b.
+Proof.
+  intros; induction IN; [econstructor 1|econstructor 2|econstructor 3]; eauto.
+Qed.
+
+Lemma tc_mon: forall X (R R': X -> X -> Prop) a b
+    (IN: tc R a b)
+    (LE: R <2= R'),
+  tc R' a b.
+Proof.
+  intros; induction IN; [econstructor 1|econstructor 2]; eauto.
+Qed.
+
+Lemma tc_rtc: forall X r (a b: X)
+    (TC: tc r a b),
+  rtc r a b.
+Proof.
+  intros; induction TC; eauto using rt_trans.
+Qed.
+
+Lemma rtc_tc: forall X r (a b: X)
+    (RTC: rtc r a b),
+  a = b \/ tc r a b.
+Proof.
+  intros; induction RTC; eauto.
+  destruct IHRTC1, IHRTC2; subst; eauto.
+  right; econstructor 2; eauto.
+Qed.
+
+Lemma tc_rtc_tc: forall X r (a b c: X)
+    (TC: tc r a b)
+    (RTC: rtc r b c),
+  tc r a c.
+Proof.
+  intros; induction RTC; eauto using t_trans, t_step.
+Qed.
+
+Lemma rtc_tc_tc: forall X r (a b c: X)
+    (RTC: rtc r a b)
+    (TC: tc r b c),
+  tc r a c.
+Proof.
+  intros; induction RTC; eauto using t_trans, t_step.
+Qed.
+
+Lemma tc_first: forall X r (a c: X)
+    (CT: tc r a c),
+  exists b, r a b /\ rtc r b c.
+Proof.
+  intros. induction CT; eauto using rt_refl; clear IHCT2.
+  destruct IHCT1 as [? []].
+  eauto using rt_step, tc_rtc, rtc_tc_tc.
+Qed.
+
+Lemma tc_last: forall X r (a c: X)
+    (CT: tc r a c),
+  exists b, rtc r a b /\ r b c.
+Proof.
+  intros; induction CT; eauto using rt_refl; clear IHCT1.
+  destruct IHCT2 as [? []].
+  eauto using rt_step, tc_rtc, tc_rtc_tc.
+Qed.
+
+(** * Definitions. *)
+
+(** **
+  Wellfounded Order
+ *)
+
+Structure bwfo :=
+  { bwfo_set :> Type;
+    bwfo_lt : bwfo_set -> bwfo_set -> Prop;
+    bwfo_le : bwfo_set -> bwfo_set -> Prop;
+
+    bwfo_le_refl: forall i, bwfo_le i i;
+    bwfo_lt_le: forall i j, bwfo_lt i j -> bwfo_le i j;
+    bwfo_le_le_le: forall i j k, bwfo_le i j -> bwfo_le j k -> bwfo_le i k;
+    bwfo_lt_le_lt: forall i j k, bwfo_lt i j -> bwfo_le j k -> bwfo_lt i k;
+    bwfo_le_lt_lt: forall i j k, bwfo_le i j -> bwfo_lt j k -> bwfo_lt i k;
+    
+    bwfo_wf : well_founded bwfo_lt;
+}.
+Arguments bwfo_lt {_} _ _.
+Arguments bwfo_le {_} _ _.
+
+(* **
+  Symmetric Product of Algebraic Wellfounded Orders
+ *)
+
+Definition symprod_lt (a b : bwfo) (x y: a * b) :=
+  (bwfo_lt (fst x) (fst y) /\ bwfo_le (snd x) (snd y)) \/
+  (bwfo_le (fst x) (fst y) /\ bwfo_lt (snd x) (snd y)).
+
+Definition symprod_le (a b : bwfo) (x y: a * b) :=
+  bwfo_le (fst x) (fst y) /\ bwfo_le (snd x) (snd y).
+
+Program Definition bwfo_symprod (a b : bwfo) : bwfo :=
+  {| bwfo_lt   := symprod_lt a b;
+     bwfo_le   := symprod_le a b;
+  |}.
+Next Obligation. split; simpl; eauto using bwfo_le_refl. Qed.
+Next Obligation.
+  destruct H as [[]|[]]; split; simpl in *; eauto using bwfo_lt_le, bwfo_le_le_le.
+Qed.
+Next Obligation.
+  destruct H, H0; split; simpl in *; eauto using bwfo_le_le_le.
+Qed.
+Next Obligation.
+  destruct H, H, H0; [left|right]; split; simpl in *; eauto using bwfo_lt_le_lt, bwfo_le_le_le.
+Qed.
+Next Obligation.
+  destruct H, H0, H0; [left|right]; split; simpl in *; eauto using bwfo_le_lt_lt, bwfo_le_le_le.
+Qed.
+Next Obligation.
+  intros [u v].
+  assert (WFu := bwfo_wf _ u). revert v.
+  induction WFu as [u _ HYPu].
+  econstructor; intros [u' v'] LT'.
+  destruct LT', H; simpl in *.
+  - eapply HYPu in H; eauto.
+  - clear v H0.
+    assert (WFv' := bwfo_wf _ v'). revert u' H.
+    induction WFv' as [v' _ HYPv'].
+    econstructor; intros [u'' v''] LT''.
+    destruct LT'', H0; simpl in *.
+    + eapply HYPu; eauto using bwfo_lt_le_lt.
+    + eapply HYPv'; eauto using bwfo_le_le_le.
+Qed.
+
+(* **
+  Lexcographic Product of Algebraic Wellfounded Orders
+ *)
+
+Definition lexprod_lt (a b : bwfo) (x y: a * b) :=
+  bwfo_lt (fst x) (fst y) \/
+  (bwfo_le (fst x) (fst y) /\ bwfo_lt (snd x) (snd y)).
+
+Definition lexprod_le (a b : bwfo) (x y: a * b) :=
+  bwfo_lt (fst x) (fst y) \/
+  (bwfo_le (fst x) (fst y) /\ bwfo_le (snd x) (snd y)).
+
+Program Definition bwfo_lexprod (a b : bwfo) : bwfo :=
+  {| bwfo_lt   := lexprod_lt a b;
+     bwfo_le   := lexprod_le a b;
+  |}.
+Next Obligation. right. split; simpl; eauto using bwfo_le_refl. Qed.
+Next Obligation.
+  destruct H as [|[]]; [left|right]; simpl in *; eauto using bwfo_lt_le.
+Qed.
+Next Obligation.
+  destruct H as [|[]], H0 as [|[]]; [..|right]; try left; simpl in *; eauto using bwfo_lt_le, bwfo_lt_le_lt, bwfo_le_lt_lt, bwfo_le_le_le.
+Qed.
+Next Obligation.
+  destruct H as [|[]], H0 as [|[]]; [..|right]; try left; simpl in *; eauto using bwfo_lt_le, bwfo_lt_le_lt, bwfo_le_lt_lt, bwfo_le_le_le.
+Qed.
+Next Obligation.
+  destruct H as [|[]], H0 as [|[]]; [..|right]; try left; simpl in *; eauto using bwfo_lt_le, bwfo_lt_le_lt, bwfo_le_lt_lt, bwfo_le_le_le.
+Qed.
+Next Obligation.
+  intros [u v].
+  assert (WFu := bwfo_wf _ u). revert v.
+  induction WFu as [u _ HYPu].
+  econstructor; intros [u' v'] LT'.
+  destruct LT' as [|[]]; simpl in *.
+  - eapply HYPu in H; eauto.
+  - clear v H0.
+    assert (WFv' := bwfo_wf _ v'). revert u' H.
+    induction WFv' as [v' _ HYPv'].
+    econstructor; intros [u'' v''] LT''.
+    destruct LT'' as [|[]]; simpl in *.
+    + eapply HYPu; eauto using bwfo_lt_le_lt.
+    + eapply HYPv'; eauto using bwfo_le_le_le.
+Qed.
+
+(** **
+  Non-trival Non-negative Well-founded Ordered Monoids
+ *)
+
+Structure awfo :=
+{ wfo_set :> Type;
+
+  wfo_zero : wfo_set;
+  wfo_add  : wfo_set -> wfo_set -> wfo_set;
+
+  wfo_lt : wfo_set -> wfo_set -> Prop;
+  wfo_le  : wfo_set -> wfo_set -> Prop;
+
+(* Monoid *)
+  
+  wfo_add_zero_l_le: forall i, wfo_le (wfo_add wfo_zero i) i;
+  wfo_add_zero_l_ge: forall i, wfo_le i (wfo_add wfo_zero i);
+  wfo_add_zero_r_le: forall i, wfo_le (wfo_add i wfo_zero) i;
+  wfo_add_zero_r_ge: forall i, wfo_le i (wfo_add i wfo_zero);
+  
+  wfo_add_assoc_le: forall i j k, wfo_le (wfo_add i (wfo_add j k)) (wfo_add (wfo_add i j) k);
+  wfo_add_assoc_ge: forall i j k, wfo_le (wfo_add (wfo_add i j) k) (wfo_add i (wfo_add j k));
+
+(* Order *)
+
+  wfo_le_refl: forall i, wfo_le i i;
+  wfo_lt_le: forall i j, wfo_lt i j -> wfo_le i j;
+  wfo_le_le_le: forall i j k, wfo_le i j -> wfo_le j k -> wfo_le i k;
+  wfo_lt_le_lt: forall i j k, wfo_lt i j -> wfo_le j k -> wfo_lt i k;
+  wfo_le_lt_lt: forall i j k, wfo_le i j -> wfo_lt j k -> wfo_lt i k;
+
+  wfo_add_le_left: forall i i' j (LE: wfo_le i i'), wfo_le (wfo_add i j) (wfo_add i' j);
+  wfo_add_le_right: forall i j j' (LE: wfo_le j j'), wfo_le (wfo_add i j) (wfo_add i j');
+  wfo_add_lt_left: forall i i' j (LT: wfo_lt i i'), wfo_lt (wfo_add i j) (wfo_add i' j);
+  wfo_add_lt_right: forall i j j' (LT: wfo_lt j j'), wfo_lt (wfo_add i j) (wfo_add i j');
+
+(* Well-founded *)
+  wfo_wf : well_founded wfo_lt;
+
+(* Positive *)
+  wfo_non_negative: forall i, wfo_le wfo_zero i;
+
+(* Non-trivial *)
+  wfo_one  : wfo_set;
+  wfo_non_trivial : wfo_lt wfo_zero wfo_one;
+}.
+
+Arguments wfo_lt {_} _ _.
+Arguments wfo_le {_} _ _.
+Arguments wfo_zero {_}.
+Arguments wfo_one {_}.
+Arguments wfo_add {_} _ _.
+
+(* **
+  General Wellfounded Order in NtNnWfPoMonoid
+ *)
+
+Definition gwf_set : Type := list (sigT bwfo_set).
+
+Definition gwfel (o: bwfo) (x: o) :=
+  existT _ o x.
+
+Program Definition unit_wfo : bwfo :=
+  {| bwfo_set := unit;
+     bwfo_lt _ _ := False;
+     bwfo_le _ _ := True;
+  |}.
+Next Obligation. econstructor; intros. contradiction. Qed.
+
+Definition gwf_one : gwf_set := 
+  [ gwfel unit_wfo tt ].
+
+Inductive gwf_lex (b: bool) : gwf_set -> gwf_set -> Prop :=
+| gwf_lex_nil
+    (CHECK: is_true b)
+  : gwf_lex b [] []
+| gwf_lex_lt
+    o x y i j
+    (LT: bwfo_lt x y)
+    (LEN: length i = length j)
+  : gwf_lex b (gwfel o x :: i) (gwfel o y :: j)
+| gwf_lex_step
+    o x y i j
+    (LE: bwfo_le x y)
+    (CMP: gwf_lex b i j)
+  : gwf_lex b (gwfel o x :: i) (gwfel o y :: j)
+.    
+Hint Constructors gwf_lex.
+
+Variant gwf_cmp b : gwf_set -> gwf_set -> Prop :=
+| gwf_cmp_lt
+    o1 o2
+    (LEN: length o1 < length o2)
+  : gwf_cmp b o1 o2
+| gwf_cmp_lex
+    i j
+    (CMP: gwf_lex b i j)
+  : gwf_cmp b i j
+.
+Hint Constructors gwf_cmp.
+
+Lemma gwf_lex_length b o1 o2
+      (LT: gwf_lex b o1 o2)
+  : length o1 = length o2.
+Proof.
+  intros. induction LT; simpl; nia.
+Qed.  
+
+Lemma gwf_cmp_length b o1 o2
+      (CMP: gwf_cmp b o1 o2)
+  : length o1 <= length o2.
+Proof.
+  destruct CMP.
+  - nia.
+  - erewrite gwf_lex_length; eauto. 
+Qed.
+
+Lemma gwf_lex_refl: forall i, gwf_lex true i i.
+Proof.
+  induction i; eauto.
+  destruct a. eapply gwf_lex_step; eauto using bwfo_le_refl.
+Qed.
+
+Lemma gwf_le_refl: forall i, gwf_cmp true i i.
+Proof.
+  intros. apply gwf_cmp_lex. eauto using gwf_lex_refl.
+Qed.
+
+Lemma gwf_lex_lt_le: forall i j, gwf_lex false i j -> gwf_lex true i j.
+Proof.
+  intros. induction H; eauto.
+Qed.
+
+Lemma gwf_lt_le: forall i j, gwf_cmp false i j -> gwf_cmp true i j.
+Proof.
+  intros. destruct H; eauto using gwf_lex_lt_le.
+Qed.
+
+Lemma gwf_lex_trans b1 b2 b3 i j k
+      (COND: is_true (b1 && b2) -> is_true b3)
+      (CMP1: gwf_lex b1 i j)
+      (CMP2: gwf_lex b2 j k)
+  : gwf_lex b3 i k.
+Proof.
+  ginduction CMP2; intros.
+  - inversion CMP1; subst. destruct b1, b2, b3; eauto.
+  - dependent destruction CMP1.
+    + eapply gwf_lex_lt; eauto using bwfo_le_lt_lt, bwfo_lt_le.
+      nia.
+    + eapply gwf_lex_lt; eauto using bwfo_le_lt_lt.
+      apply gwf_lex_length in CMP1. nia.
+  - dependent destruction CMP1.
+    + eapply gwf_lex_lt; eauto using bwfo_lt_le_lt.
+      apply gwf_lex_length in CMP2. nia.
+    + eapply gwf_lex_step; eauto using bwfo_le_le_le.
+Qed.
+
+Lemma gwf_cmp_trans b1 b2 b3 i j k
+      (CMP1: gwf_cmp b1 i j)
+      (CMP2: gwf_cmp b2 j k)
+      (COND: is_true (b1 && b2) -> is_true b3)
+  : gwf_cmp b3 i k.
+Proof.
+  assert (LE1 := gwf_cmp_length CMP1).
+  assert (LE2 := gwf_cmp_length CMP2).
+  destruct CMP1, CMP2; eauto using gwf_lex_trans; apply gwf_cmp_lt; nia.
+Qed.
+
+Lemma gwf_add_cmp_left b: forall i i' j (LE: gwf_cmp b i i'), gwf_cmp b (i ++ j) (i' ++ j).
+Proof.
+  intros. inversion LE; subst.
+  - apply gwf_cmp_lt. rewrite !app_length. nia.
+  - apply gwf_cmp_lex.
+    induction CMP; simpl.
+    + destruct b; inversion CHECK. eauto using gwf_lex_refl.
+    + apply gwf_lex_lt; eauto.
+      rewrite !app_length. nia.
+    + apply gwf_lex_step; eauto.
+Qed.
+
+Lemma gwf_add_cmp_right b: forall i j j' (LE: gwf_cmp b j j'), gwf_cmp b (i ++ j) (i ++ j').
+Proof.
+  intros. inversion LE; subst.
+  - apply gwf_cmp_lt. rewrite !app_length. nia.
+  - apply gwf_cmp_lex.
+    ginduction CMP; simpl; intros.
+    + destruct b; inversion CHECK. eauto using gwf_lex_refl.
+    + induction i0; simpl; eauto.
+      destruct a; eauto using bwfo_le_refl.
+    + induction i0; simpl; eauto.
+      destruct a; eauto using bwfo_le_refl.
+Qed.
+
+Lemma gwf_acc_le: forall i j (WF: Acc (gwf_cmp false) i) (LE: gwf_cmp true j i),
+    Acc (gwf_cmp false) j.
+Proof.
+  econstructor. intros. eapply WF. eauto using gwf_cmp_trans.
+Qed.
+
+Lemma gwf_lt_bottom: forall i, gwf_cmp false i [] -> False.
+Proof.
+  intros. inversion H; subst.
+  - inversion LEN.
+  - inversion CMP. inversion CHECK.
+Qed.
+       
+Lemma gwf_wf: well_founded (gwf_cmp false).
+Proof.
+  cut (forall n i (LEon: length i <= n), Acc (gwf_cmp false) i).
+  { red; eauto. }
+
+  induction n; intros.
+  { destruct i; inversion LEon.
+    econstructor. intros. exfalso. eauto using gwf_lt_bottom. }
+  destruct i.
+  { econstructor. intros. exfalso. eauto using gwf_lt_bottom. }
+
+  destruct s as [o x]. revert i LEon. simpl.
+  assert (WFx := bwfo_wf _ x).
+  induction WFx as [x _ HYPx].
+  econstructor. intros j LTj.
+  dependent destruction LTj.
+  { simpl in *. eapply IHn. nia. }
+  dependent destruction CMP.
+  { eapply HYPx; eauto. nia. }
+  
+  assert (WF: Acc (gwf_cmp false) i0).
+  { apply gwf_lex_length in CMP. eapply IHn. nia. }
+  revert x0 LE. induction WF as [j _ HYPj].
+  econstructor. intros k LTk.
+  assert (LEN := gwf_lex_length CMP).
+  dependent destruction LTk.
+  { simpl in *. eapply IHn. nia. }
+  dependent destruction CMP0.
+  { eapply HYPx; eauto using bwfo_lt_le_lt. nia. }
+  eapply HYPj; eauto using bwfo_le_le_le.
+  eapply gwf_lex_trans; eauto; eauto.
+Qed.
+
+Program Definition gwfo : awfo :=
+  {| wfo_set     := gwf_set;
+     wfo_le x y  := gwf_cmp true x y;
+     wfo_lt x y  := gwf_cmp false x y;
+     wfo_zero    := nil;
+     wfo_one     := gwf_one;
+     wfo_add x y := x ++ y;
+  |}.
+Next Obligation. eauto using gwf_le_refl. Qed.
+Next Obligation. eauto using gwf_le_refl. Qed.
+Next Obligation. rewrite app_nil_r. eauto using gwf_le_refl. Qed.
+Next Obligation. rewrite app_nil_r. eauto using gwf_le_refl. Qed.
+Next Obligation. rewrite app_assoc. eauto using gwf_le_refl. Qed.
+Next Obligation. rewrite app_assoc. eauto using gwf_le_refl. Qed.
+Next Obligation. eauto using gwf_le_refl. Qed.
+Next Obligation. eauto using gwf_lt_le. Qed.
+Next Obligation. eauto using gwf_cmp_trans. Qed.
+Next Obligation. eauto using gwf_cmp_trans. Qed.
+Next Obligation. eauto using gwf_cmp_trans. Qed.
+Next Obligation. eauto using gwf_add_cmp_left. Qed.
+Next Obligation. eauto using gwf_add_cmp_right. Qed.
+Next Obligation. eauto using gwf_add_cmp_left. Qed.
+Next Obligation. eauto using gwf_add_cmp_right. Qed.
+Next Obligation. eauto using gwf_wf. Qed.
+Next Obligation. destruct i; eauto. econstructor. simpl. nia. Qed.
+
+(* **
+   embedding and properties
+ *)
+
+Definition gwf_embed {o: bwfo} (a: o) : gwfo :=
+  [ gwfel o a ].
+
+Lemma gwf_embed_le_preserve (o: bwfo) (a b: o)
+      (LT: bwfo_le a b):
+  wfo_le (gwf_embed a) (gwf_embed b).
+Proof.
+  repeat red. unfold gwf_embed. eauto.
+Qed.
+
+Lemma gwf_embed_lt_preserve (o: bwfo) (a b: o)
+      (LT: bwfo_lt a b):
+  wfo_lt (gwf_embed a) (gwf_embed b).
+Proof.
+  repeat red. unfold gwf_embed. eauto.
+Qed.
+
+Lemma gwf_embed_reflect (o: bwfo) (a b: o)
+    (LT: wfo_lt (gwf_embed a) (gwf_embed b)):
+  bwfo_lt a b.
+Proof.
+  repeat red in LT. unfold gwf_embed in *. dependent destruction LT; eauto.
+  - simpl in *. nia.
+  - dependent destruction CMP; eauto.
+    inversion CMP. inversion CHECK.
+Qed.
+
+(* **
+  Simple Properties about Orders
+ *)
+
+Lemma wfo_lt_neq: forall a i, ~ @wfo_lt a i i.
+Proof.
+  intros. assert (WF := wfo_wf a i). red.
+  induction WF. eauto.
+Qed.
+
+Lemma wfo_add_monotone: forall (a: awfo) (i i' j j': a)
+    (LEi: wfo_le i i')
+    (LEj: wfo_le j j'),
+  wfo_le (wfo_add i j) (wfo_add i' j').
+Proof.
+  eauto using wfo_le_le_le, wfo_add_le_left, wfo_add_le_right. 
+Qed.
+
+Lemma wfo_add_proj_left: forall a i j, @wfo_le a i (wfo_add i j).
+Proof.
+  eauto using wfo_le_le_le, wfo_add_zero_r_ge, wfo_add_le_right, wfo_non_negative.
+Qed.
+
+Lemma wfo_add_proj_right: forall a i j, @wfo_le a j (wfo_add i j).
+Proof.
+  eauto using wfo_le_le_le, wfo_add_zero_l_ge, wfo_add_le_left, wfo_non_negative.
+Qed.
+
+Lemma wfo_add_one: forall (a: awfo) (i: a), wfo_lt i (wfo_add wfo_one i).
+Proof.
+  eauto using wfo_le_lt_lt, wfo_add_proj_right, wfo_add_lt_left, wfo_non_trivial.  
+Qed.
+
+(** [wfo_le_n n o o'] means that [o'] can be decreased at least [n] times
+    before reaching [o].
+*)
+Inductive wfo_le_n {o: awfo} : nat -> o -> o -> Prop :=
+| wfo_le_n_Z i j (LE: wfo_le i j)
+  : wfo_le_n O i j
+| wfo_le_n_S n i j k (GLE: wfo_le_n n i j) (LT: wfo_lt j k)
+  : wfo_le_n (S n) i k
+.
+Hint Constructors wfo_le_n.
+
+Lemma wfo_le_n_lt: forall o n (i i': wfo_set o)
+    (LE: wfo_le_n (S n) i i'),
+  wfo_lt i i'.
+Proof.
+  induction n; intros; inversion LE; subst.
+  - inversion GLE; subst. eauto using wfo_le_lt_lt.
+  - apply IHn in GLE. eauto using wfo_lt_le, wfo_lt_le_lt.
+Qed.
+
+(* TODO rename (D) *)
+Lemma wfo_le_n_S': forall o n (i i': wfo_set o)
+    (LE: wfo_le_n (S n) i i'),
+  exists j : wfo_set o,
+    wfo_lt i j /\
+    wfo_le_n n j i'.
+Proof.
+  induction n; intros; inversion LE; subst.
+  - inversion GLE. subst. eauto using wfo_le_lt_lt, wfo_le_refl. 
+  - edestruct IHn; eauto.
+    destruct H. eauto.
+Qed.
+
+Lemma wfo_le_n_S'': forall o n (i i': wfo_set o)
+    (LE: wfo_le_n (S n) i i'),
+  wfo_le_n n i i'.
+Proof.
+  intros; inversion LE; inversion GLE; subst; eauto using wfo_lt_le, wfo_le_le_le, wfo_lt_le_lt.
+Qed.
+
+Lemma wfo_le_n_wfo_le: forall o n (i i' i'': wfo_set o)
+    (GLE: wfo_le_n n i i')
+    (LE: wfo_le i' i''),
+  wfo_le_n n i i''.
+Proof.
+  intros; dependent destruction GLE; [econstructor 1|econstructor 2]; eauto using wfo_le_le_le, wfo_lt_le_lt.
+Qed.
+
+Lemma wfo_le_n_anti: forall o m n (i i': wfo_set o)
+    (GLE: wfo_le_n m i i')
+    (LE: n <= m),
+  wfo_le_n n i i'.
+Proof.
+  intros; ginduction LE; eauto.
+  intros; apply IHLE; auto using wfo_le_n_S''.
+Qed.
+
+(* TODO rename *)
+Lemma wfo_le_n_S_rev: forall o (i j: wfo_set o) n k
+    (LT: wfo_lt i j)
+    (GLE: wfo_le_n n j k),
+  wfo_le_n (S n) i k.
+Proof.
+  intros; ginduction GLE; intros; eauto.
+  econstructor; eauto using wfo_lt_le_lt, wfo_le_refl.
+Qed.
+
+Lemma wfo_le_n_plus: forall o n na nb (i i': wfo_set o)
+    (GLE: wfo_le_n n i i')
+    (E: n = na + nb),
+  exists ii,
+    wfo_le_n na i ii /\
+    wfo_le_n nb ii i'.
+Proof.
+  intros; ginduction na; simpl; intros; subst.
+  - exists i; eauto using wfo_le_refl.
+  - apply wfo_le_n_S' in GLE. destruct GLE as [? [? LE]].
+    eapply IHna in LE; eauto.
+    destruct LE as [ii []].
+    exists ii; eauto; split; eauto using wfo_le_n_S_rev.
+Qed.
+
+(* **
+  wfo_nat  
+*)
+
+Fixpoint wfo_nat {o : awfo} (n: nat) : wfo_set o :=
+  match n with
+  | 0 => wfo_zero
+  | S n' => wfo_add wfo_one (wfo_nat n')
+  end.
+
+Lemma wfo_le_n_add: forall o n (i: wfo_set o),
+  wfo_le_n n i (wfo_add (wfo_nat n) i).
+Proof.
+  induction n; eauto using wfo_add_lt_left, wfo_add_one, wfo_le_refl, wfo_add_proj_right.
+Qed.
+
+Lemma wfo_nat_le_mon: forall o n m
+    (LE: n <= m),
+  @wfo_le o (wfo_nat n) (wfo_nat m).
+Proof.
+  intros. induction LE; eauto using wfo_le_le_le, wfo_add_proj_right, wfo_le_refl.
+Qed.
+
+Lemma wfo_nat_lt_mon: forall o n m
+    (LE: n < m),
+  @wfo_lt o (wfo_nat n) (wfo_nat m).
+Proof.
+  intros; induction LE; eauto using wfo_lt_le_lt, wfo_lt_le, wfo_add_one.
+Qed.
